cleanup, restructuring, coqdoc, todos done

coq/heytingarithmetic.v
@@ -1,19 +1,27 @@
-Require Import Coq.omega.Omega.
+(**
+* Heyting arithmetic
+*)
 
-Require Import myvec.
+Require Import Coq.Setoids.Setoid.
+
+Require Import fin.
+Require Import vec.
 
 Import FIN.NOTATIONS.
 Import VEC.NOTATIONS.
-
 
 Local Open Scope FIN.
 Local Open Scope VEC.
 
 Module HA.
 
-  (**********)
-  (* SYNTAX *)
-  (**********)
+  (**
+  ** Syntax
+  *)
+
+  (**
+  *** Terms
+  *)
 
   Inductive term (n : nat) :=
   | O'    : term n
@@ -29,26 +37,34 @@ Module HA.
   Local Infix "﬩" := plus' (at level 64).
   Local Infix "⋅" := mult' (at level 63).
 
-  Definition x11 : term 1 := var (FIN.ofNat 0 0).
-  Definition x12 : term 2 := var (FIN.ofNat 0 1).
-  Definition x22 : term 2 := var (FIN.ofNat 1 0).
-  Definition x13 : term 3 := var (FIN.ofNat 0 2).
-  Definition x23 : term 3 := var (FIN.ofNat 1 1).
-  Definition x33 : term 3 := var (FIN.ofNat 2 0).
-  Definition x14 : term 4 := var (FIN.ofNat 0 3).
-  Definition x24 : term 4 := var (FIN.ofNat 1 2).
-  Definition x34 : term 4 := var (FIN.ofNat 2 1).
-  Definition x44 : term 4 := var (FIN.ofNat 3 0).
+  Definition x01 : term 1 := var (FIN.ofNat 0 0).
+  Definition x02 : term 2 := var (FIN.ofNat 0 1).
+  Definition x12 : term 2 := var (FIN.ofNat 1 0).
+  Definition x03 : term 3 := var (FIN.ofNat 0 2).
+  Definition x13 : term 3 := var (FIN.ofNat 1 1).
+  Definition x23 : term 3 := var (FIN.ofNat 2 0).
+  Definition x04 : term 4 := var (FIN.ofNat 0 3).
+  Definition x14 : term 4 := var (FIN.ofNat 1 2).
+  Definition x24 : term 4 := var (FIN.ofNat 2 1).
+  Definition x34 : term 4 := var (FIN.ofNat 3 0).
+
+  (**
+  *** Atomic formulas
+  *)
 
   Inductive atom (n : nat) :=
-    FF     : atom n
+  | FF     : atom n
   | atomEq : term n -> term n -> atom n.
   Arguments FF {_}.
   Arguments atomEq {_} _ _.
   Local Infix "≐" := atomEq (at level 65).
 
+  (**
+  *** Formulas
+  *)
+
   Inductive formula n :=
-    fAtom : atom n -> formula n
+  | fAtom : atom n -> formula n
   | fAnd  : formula n -> formula n -> formula n
   | fOr   : formula n -> formula n -> formula n
   | fImp  : formula n -> formula n -> formula n
@@ -69,9 +85,37 @@ Module HA.
   Local Notation "∃ A" := (fEx A) (at level 5).
   Local Notation "∀ A" := (fFa A) (at level 5).
 
-  (****************)
-  (* SUBSTITUTION *)
-  (****************)
+  (**
+  *** Term promotion
+  *)
+
+  Fixpoint termUp {n : nat} (t : term n) : term (S n) :=
+  match t with
+  | O'    => O'
+  | var x => var ++x
+  | S' t  => S' (termUp t)
+  | u ﬩ v => (termUp u) ﬩ (termUp v)
+  | u ⋅ v => (termUp u) ⋅ (termUp v)
+  end.
+
+  Definition termVecUp {n m} (f : VEC.t (term m) n) : VEC.t (term (S m)) n :=
+    VEC.map termUp f.
+
+  (**
+  *** Identity term vectors
+  *)
+
+  Definition idVec {n} : VEC.t (term n) n := VEC.finMap var.
+
+  Definition idVecUp {n} : VEC.t (term (S n)) n := VEC.finMap' (k := 1) var.
+
+  (**
+  ** Substitution
+  *)
+
+  (**
+  *** Substitution in terms
+  *)
 
   Fixpoint termSubst {n m} (t : term n) (f : VEC.t (term m) n) : term m :=
   match t with
@@ -82,147 +126,124 @@ Module HA.
   | u ⋅ v => termSubst u f ⋅ termSubst v f
   end.
 
+  (**
+  *** Substitution in atoms
+  *)
+
   Definition atomSubst {n m} (A : atom n) (f : VEC.t (term m) n) : atom m :=
   match A with
   | FF    => FF
   | u ≐ v => termSubst u f ≐ termSubst v f
   end.
 
-  Fixpoint termUp {n : nat} (t : term n) : term (S n) := match t with
-  | O'    => O'
-  | var x => var ++x
-  | S' t  => S' (termUp t)
-  | u ﬩ v => (termUp u) ﬩ (termUp v)
-  | u ⋅ v => (termUp u) ⋅ (termUp v)
-  end.
+  (**
+  *** Substitution in formulas
+  *)
 
-  Definition termVecUp {n m : nat} (f : VEC.t (term m) n)
-    : VEC.t (term (S m)) n := (VEC.map termUp f).
-
-  Definition termVecUp' {n m : nat} (f : VEC.t (term m) n)
-    : VEC.t (term (S m)) (S n) := (termVecUp f, var FIN.last).
-
-  Definition idVec {n} : VEC.t (term n) n := VEC.finMap var.
-
-  Definition idVecUp {n} : VEC.t (term (S n)) n := VEC.finMap' (k := 1) var.
-
-  Fixpoint formulaSubstitution {n m} (A : formula n) (f : VEC.t (term m) n)
+  Fixpoint formulaSubst {n m} (A : formula n) (f : VEC.t (term m) n)
     : formula m :=
   match A with
   | fAtom A => atomSubst A f
-  | A ∧ B   => formulaSubstitution A f ∧ formulaSubstitution B f
-  | A ∨ B   => formulaSubstitution A f ∨ formulaSubstitution B f
-  | A → B   => formulaSubstitution A f → formulaSubstitution B f
-  | ∃A      => ∃(formulaSubstitution A (termVecUp' f))
-  | ∀A      => ∀(formulaSubstitution A (termVecUp' f))
+  | A ∧ B   => formulaSubst A f ∧ formulaSubst B f
+  | A ∨ B   => formulaSubst A f ∨ formulaSubst B f
+  | A → B   => formulaSubst A f → formulaSubst B f
+  | ∃A      => ∃(formulaSubst A ((termVecUp f), var FIN.last))
+  | ∀A      => ∀(formulaSubst A ((termVecUp f), var FIN.last))
   end.
-  Local Infix "//" := formulaSubstitution (at level 62, left associativity).
+  Local Infix "//" := formulaSubst (at level 62, left associativity).
 
-  Definition lastSubstitution {n} (A : formula (S n)) (t : term (S n))
-    : formula (S n) := A // (idVecUp, t).
-  Local Infix "/+" := lastSubstitution (at level 62, left associativity).
+  (**
+  *** Substitution in the last variable
+  *)
 
-  Definition downSubstitution {n} (A : formula (S n)) (t : term n)
-    : formula n := A // (idVec, t).
-  Local Infix "/-" := downSubstitution (at level 62, left associativity).
+  Definition lastSubst {n} (A : formula (S n)) (t : term (S n)) : formula (S n)
+    := A // (idVecUp, t).
+  Local Infix "/+" := lastSubst (at level 62, left associativity).
+
+  Definition downSubst {n} (A : formula (S n)) (t : term n) : formula n :=
+    A // (idVec, t).
+  Local Infix "/-" := downSubst (at level 62, left associativity).
+
+  (**
+  *** Formula promotion
+  *)
 
   Definition formulaUp {n} (A : formula n) : formula (S n) := A // idVecUp.
-
   Local Notation up := formulaUp.
 
-  (*************)
-  (* SEMANTICS *)
-  (*************)
+  (**
+  ** Semantics
+  *)
 
-  Class Model (Truth : forall {n}, formula n -> Prop) := {
+  Class Interpretation (Truth : forall {n}, formula n -> Prop) := {
     Consistency : ~Truth (@FF 0);
-
     RuleMP {n} (A B : formula n) : Truth (A → B) -> Truth A -> Truth B;
-
     RuleGen {n} (A : formula (S n)) : Truth A -> Truth ∀A;
-
     RuleUp {n} (A : formula n) : Truth A -> Truth (up A);
-
     AxImp1 {n} (A B : formula n) : Truth (A → B → A);
-
     AxImp2 {n} (A B C : formula n) : Truth ((A → B → C) → (A → B) → A → C);
-
     AxAndI {n} (A B : formula n) : Truth (A → B → A ∧ B);
-
     AxAndE1 {n} (A B : formula n) : Truth (A ∧ B → A);
-
     AxAndE2 {n} (A B : formula n) : Truth (A ∧ B → B);
-
     AxOrI1 {n} (A B : formula n) : Truth (A → A ∨ B);
-
     AxOrI2 {n} (A B : formula n) : Truth (B → A ∨ B);
-
     AxOrE {n} (A B C : formula n) : Truth (A ∨ B → (A → C) → (B → C) → C);
-
     AxExFalso {n} (A : formula n) : Truth (FF → A);
-
-    AxExI {n} (A : formula (S n)) (t : term n) : Truth (A /- t → ∃A);
-
+    AxExI {n} (A : formula (S n)) (t : term n) : Truth (A/-t → ∃A);
     AxExE {n} (A : formula (S n)) (B : formula n) :
       Truth (∀(A → up B) → ∃A → B);
-
     AxFaI {n} (A : formula n) (B : formula (S n)) :
       Truth (∀(up A → B) → A → ∀B);
-
-    AxFaE {n} (A : formula (S n)) (t : term n) : Truth (∀A → A /- t);
-
-    AxEqRefl : Truth (x11 ≐ x11);
-
-    AxEqSymm : Truth (x12 ≐ x22 → x22 ≐ x12);
-
-    AxEqTrans : Truth (x13 ≐ x23 → x23 ≐ x33 → x13 ≐ x33);
-
-    AxEqS : Truth (x12 ≐ x22 → S' x12 ≐ S' x22);
-
-    AxEqPlus : Truth (x14 ≐ x24 → x34 ≐ x44 → x14 ﬩ x34 ≐ x24 ﬩ x44);
-
-    AxEqMult : Truth (x14 ≐ x24 → x34 ≐ x44 → x14 ⋅ x34 ≐ x24 ⋅ x44);
-
-    AxPA1 : Truth (S' x11 ≠ x11);
-
-    AxPA2 : Truth (S' x12 ≐ S' x22 → x12 ≐ x22);
-
-    AxPA3 : Truth (x11 ﬩ O' ≐ x11);
-
-    AxPA4 : Truth (x12 ﬩ S' x22 ≐ S' (x12 ﬩ x22));
-
-    AxPA5 : Truth (x11 ⋅ O' ≐ O');
-
-    AxPA6 : Truth (x12 ⋅ S' x22 ≐ x12⋅x22 ﬩ x12);
-
+    AxFaE {n} (A : formula (S n)) (t : term n) : Truth (∀A → A/-t);
+    AxEqRefl : Truth (x01 ≐ x01);
+    AxEqSymm : Truth (x02 ≐ x12 → x12 ≐ x02);
+    AxEqTrans : Truth (x03 ≐ x13 → x13 ≐ x23 → x03 ≐ x23);
+    AxEqS : Truth (x02 ≐ x12 → S' x02 ≐ S' x12);
+    AxEqPlus : Truth (x04 ≐ x14 → x24 ≐ x34 → x04 ﬩ x24 ≐ x14 ﬩ x34);
+    AxEqMult : Truth (x04 ≐ x14 → x24 ≐ x34 → x04 ⋅ x24 ≐ x14 ⋅ x34);
+    AxPA1 : Truth (S' x01 ≠ x01);
+    AxPA2 : Truth (S' x02 ≐ S' x12 → x02 ≐ x12);
+    AxPA3 : Truth (x01 ﬩ O' ≐ x01);
+    AxPA4 : Truth (x02 ﬩ S' x12 ≐ S' (x02 ﬩ x12));
+    AxPA5 : Truth (x01 ⋅ O' ≐ O');
+    AxPA6 : Truth (x02 ⋅ S' x12 ≐ x02⋅x12 ﬩ x02);
     AxPA7 {n} (A : formula (S n)) :
-      Truth (A /- O' → ∀(A → A/+(S' (var FIN.last))) → ∀A)
+      Truth (A/-O' → ∀(A → A/+(S' (var FIN.last))) → ∀A)
   }.
 
-  Definition Provable {n} (A : formula n) :=
-    forall Truth (M : Model Truth), Truth n A.
+  (**
+  ** Standard interpretation
+  *)
 
-  (******************)
-  (* STANDARD MODEL *)
-  (******************)
+  (**
+  *** Standard term valuation
+  *)
 
-  Fixpoint standardValuation {n} (t : term n) : VEC.t nat n -> nat :=
+  Fixpoint standardVal {n} (t : term n) : VEC.t nat n -> nat :=
   match t with
   | O'     => fun _ => 0
   | var x  => fun f => VEC.nth f x
-  | S' t   => fun f => S (standardValuation t f)
-  | u ﬩ v  => fun f => standardValuation u f + standardValuation v f
-  | u ⋅ v  => fun f => standardValuation u f * standardValuation v f
+  | S' t   => fun f => S (standardVal t f)
+  | u ﬩ v  => fun f => standardVal u f + standardVal v f
+  | u ⋅ v  => fun f => standardVal u f * standardVal v f
   end.
 
-  Definition vecStandardValuation {n m} (f : VEC.t (term m) n) (g : VEC.t nat m)
-    : VEC.t nat n := VEC.map (fun t => standardValuation t g) f.
+  Definition standardVecVal {n m} (f : VEC.t (term m) n) (g : VEC.t nat m) :
+    VEC.t nat n := VEC.map (fun t => standardVal t g) f.
+
+  (**
+  *** Standard atomic truth
+  *)
 
   Definition AtomicStandardTruthPred {n} (A : atom n) : VEC.t nat n -> Prop :=
   match A with
   | FF    => fun _ => False
-  | u ≐ v => fun f => (standardValuation u f) = (standardValuation v f)
+  | u ≐ v => fun f => (standardVal u f) = (standardVal v f)
   end.
+
+  (**
+  *** Standard truth
+  *)
 
   Fixpoint StandardTruthPred {n} (A : formula n) : VEC.t nat n -> Prop :=
   match A with
@@ -234,22 +255,25 @@ Module HA.
   | ∀A      => fun f => forall x : nat, StandardTruthPred A (f, x)
   end.
 
-  Lemma idVecValuationLemma {n} (f : VEC.t nat n) :
-    vecStandardValuation idVec f = f.
+  Definition StandardTruth {n} (A : formula n) : Prop :=
+    forall f : VEC.t nat n, StandardTruthPred A f.
+
+  Lemma standardVecValIdVecEq {n} (f : VEC.t nat n) :
+    standardVecVal idVec f = f.
   Proof.
-    unfold idVec, vecStandardValuation. rewrite VEC.finMapCompose. simpl.
-    apply VEC.pointwiseEquality, VEC.finMapNth.
+    unfold idVec, standardVecVal. rewrite VEC.finMapComposeEq. simpl.
+    apply VEC.pointwiseEquality, VEC.nthFinMapEq.
   Qed.
 
-  Lemma idVecUpValuationLemma {n} (f : VEC.t nat n) (x : nat) :
-    vecStandardValuation idVecUp (f;; x) = f.
+  Lemma standardVecValIdVecUpEq {n} (f : VEC.t nat n) (x : nat) :
+    standardVecVal idVecUp (f, x) = f.
   Proof.
-    unfold idVecUp, vecStandardValuation. rewrite VEC.finMapCompose'. simpl.
-    apply VEC.pointwiseEquality, VEC.finMapNth.
+    unfold idVecUp, standardVecVal. rewrite VEC.finMapComposeEq'. simpl.
+    apply VEC.pointwiseEquality, VEC.nthFinMapEq.
   Qed.
 
-  Lemma termUpValuationLemma {n} (t : term n) (f : VEC.t nat n) (x : nat) :
-    standardValuation (termUp t) (f;; x) = standardValuation t f.
+  Lemma standardValTermUpEq {n} (t : term n) (f : VEC.t nat n) (x : nat) :
+    standardVal (termUp t) (f, x) = standardVal t f.
   Proof.
     induction t as [a | y | t IH | u IHu v IHv | u IHu v IHv]; simpl.
     - reflexivity.
@@ -259,130 +283,147 @@ Module HA.
     - rewrite IHu, IHv. reflexivity.
   Qed.
 
-  Lemma termVecUpValuationLemma {n m} (f : VEC.t (term m) n)
-                                (g : VEC.t nat m) (x : nat) :
-    vecStandardValuation (termVecUp f) (g;; x) =
-    vecStandardValuation f g.
+  Lemma standardVecValTermVecUpEq {n m} (f : VEC.t (term m) n)
+                                  (g : VEC.t nat m) (x : nat) :
+    standardVecVal (termVecUp f) (g, x) = standardVecVal f g.
   Proof.
-    setoid_rewrite VEC.mapCompose.
+    setoid_rewrite VEC.mapComposeEq.
     apply VEC.mapRespectful.
-    intro t. apply termUpValuationLemma.
+    intro t. apply standardValTermUpEq.
   Qed.
 
-  Lemma termVecUpValuationLemma' {n m} (f : VEC.t (term m) n)
-                                 (g : VEC.t nat m) (x : nat) :
-    vecStandardValuation (termVecUp' f) (g;; x) =
-    (vecStandardValuation f g;; x).
+  Lemma standardVecValTermVecUpEq' {n m} (f : VEC.t (term m) n)
+                                   (g : VEC.t nat m) (x : nat) :
+    standardVecVal (termVecUp f;; var FIN.last) (g;; x) =
+    (standardVecVal f g;; x).
   Proof.
     assert
-      (vecStandardValuation (termVecUp' f) (g;; x) =
-       (vecStandardValuation (termVecUp f) (g;; x), x))
+      (standardVecVal (termVecUp f;; var FIN.last) (g;; x) =
+       (standardVecVal (termVecUp f) (g;; x), x))
     as H by reflexivity.
     setoid_rewrite H. clear H.
-    rewrite termVecUpValuationLemma.
+    rewrite standardVecValTermVecUpEq.
     reflexivity.
   Qed.
 
-  Lemma termSubstitionLemma {n m} (t : term n) (f : VEC.t (term m) n)
-                            (g : VEC.t nat m) :
-    standardValuation (termSubst t f) g =
-    standardValuation t (vecStandardValuation f g).
+  Lemma standardValTermSubstEq {n m} (t : term n) (f : VEC.t (term m) n)
+                               (g : VEC.t nat m) :
+    standardVal (termSubst t f) g = standardVal t (standardVecVal f g).
   Proof.
     induction t as [a | x | t IH | u IHu v IHv | u IHu v IHv]; simpl.
     - reflexivity.
-    - setoid_rewrite VEC.mapNth. reflexivity.
+    - unfold standardVecVal. rewrite VEC.nthMapEq. reflexivity.
     - rewrite IH. reflexivity.
     - rewrite IHu, IHv. reflexivity.
     - rewrite IHu, IHv. reflexivity.
   Qed.
 
-  Lemma atomSubstitutionLemma {n m} (A : atom n) (f : VEC.t (term m) n)
-                              (g : VEC.t nat m) :
+  Lemma atomicTruthSubstEq {n m} (A : atom n) (f : VEC.t (term m) n)
+                           (g : VEC.t nat m) :
     AtomicStandardTruthPred (atomSubst A f) g <->
-    AtomicStandardTruthPred A (vecStandardValuation f g).
+    AtomicStandardTruthPred A (standardVecVal f g).
   Proof.
     destruct A as [ | u v]; simpl.
     - tauto.
-    - setoid_rewrite termSubstitionLemma. tauto.
+    - setoid_rewrite standardValTermSubstEq. tauto.
   Qed.
 
-  Lemma substitutionLemma {n m} (A : formula n) (f : VEC.t (term m) n)
-                          (g : VEC.t nat m) :
-    StandardTruthPred (A // f) g <->
-    StandardTruthPred A (vecStandardValuation f g).
+  Lemma standardTruthSubstEq {n m} (A : formula n) (f : VEC.t (term m) n)
+                             (g : VEC.t nat m) :
+    StandardTruthPred (A // f) g <-> StandardTruthPred A (standardVecVal f g).
   Proof.
     generalize dependent m.
     induction A as
       [n A | n A IHA B IHB | n A IHA B IHB | n A IHA B IHB | n A IH | n A IH];
-    intros m f g; simpl.
-    - apply atomSubstitutionLemma.
+      intros m f g; simpl.
+    - apply atomicTruthSubstEq.
     - rewrite IHA, IHB. tauto.
     - rewrite IHA, IHB. tauto.
     - rewrite IHA, IHB. tauto.
-    - setoid_rewrite IH. setoid_rewrite termVecUpValuationLemma'. tauto.
-    - setoid_rewrite IH. setoid_rewrite termVecUpValuationLemma'. tauto.
+    - setoid_rewrite IH. setoid_rewrite standardVecValTermVecUpEq'. tauto.
+    - setoid_rewrite IH. setoid_rewrite standardVecValTermVecUpEq'. tauto.
   Qed.
 
-  Lemma lastSubstitutionLemma {n} (A : formula (S n)) (t : term (S n))
-                              (f : VEC.t nat n) (x : nat) :
+  Lemma standardTruthLastSubstEq {n} (A : formula (S n)) (t : term (S n))
+                                 (f : VEC.t nat n) (x : nat) :
     StandardTruthPred (A /+ t) (f, x) <->
-    StandardTruthPred A (f, standardValuation t (f, x)).
+    StandardTruthPred A (f, standardVal t (f, x)).
   Proof.
-    setoid_rewrite substitutionLemma.
+    setoid_rewrite standardTruthSubstEq.
     assert
-      (vecStandardValuation (idVecUp;; t) (f;; x) =
-       (vecStandardValuation idVecUp (f;; x));; standardValuation t (f;; x))
+      (standardVecVal (idVecUp;; t) (f;; x) =
+       (standardVecVal idVecUp (f;; x));; standardVal t (f;; x))
     as H by reflexivity.
     setoid_rewrite H. clear H.
-    rewrite idVecUpValuationLemma.
+    rewrite standardVecValIdVecUpEq.
     tauto.
   Qed.
 
-  Lemma downSubstitutionLemma {n} (A : formula (S n)) (t : term n)
-                              (f : VEC.t nat n) :
-    StandardTruthPred (A /- t) f <->
-    StandardTruthPred A (f, standardValuation t f).
+  Lemma standardTruthDownSubstEq {n} (A : formula (S n)) (t : term n)
+                                 (f : VEC.t nat n) :
+    StandardTruthPred (A /- t) f <-> StandardTruthPred A (f, standardVal t f).
   Proof.
-    setoid_rewrite substitutionLemma.
+    setoid_rewrite standardTruthSubstEq.
     assert
-      (vecStandardValuation (idVec;; t) f =
-       (vecStandardValuation idVec f;; standardValuation t f))
+      (standardVecVal (idVec;; t) f = (standardVecVal idVec f, standardVal t f))
     as H by reflexivity.
     setoid_rewrite H. clear H.
-    rewrite idVecValuationLemma.
+    rewrite standardVecValIdVecEq.
     tauto.
   Qed.
 
-  Lemma upLemma {n} (A : formula n) (f : VEC.t nat n) (x : nat) :
+  Lemma standardTruthUpEq {n} (A : formula n) (f : VEC.t nat n) (x : nat) :
     StandardTruthPred (up A) (f, x) <-> StandardTruthPred A f.
   Proof.
-    unfold up. rewrite substitutionLemma, idVecUpValuationLemma. tauto.
+    unfold up. rewrite standardTruthSubstEq, standardVecValIdVecUpEq. tauto.
   Qed.
 
-  Definition StandardTruth {n} (A : formula n) : Prop :=
-    forall f : VEC.t nat n, StandardTruthPred A f.
-
-  Instance standardModel : Model (@StandardTruth).
+  Instance standardModel : Interpretation (@StandardTruth).
   Proof.
-    try omega.
-    split;
-    try (intro f; simpl; auto; try congruence; try firstorder; try omega; fail).
+    split; unfold StandardTruth; simpl.
     - intro H. exact (H ()).
-    - intros n A H [f x]. apply upLemma. apply H.
-    - intros n A t f. simpl. rewrite downSubstitutionLemma. eauto.
-    - intros n A B f. simpl. setoid_rewrite upLemma. firstorder.
-    - intros n A B f. simpl. setoid_rewrite upLemma. eauto.
-    - intros n A t f. simpl. rewrite downSubstitutionLemma. eauto.
-    - intros n A f. simpl. rewrite downSubstitutionLemma. simpl. intros H IH x.
+    - firstorder.
+    - firstorder.
+    - intros n A H [f x]. apply standardTruthUpEq. apply H.
+    - tauto.
+    - tauto.
+    - tauto.
+    - tauto.
+    - tauto.
+    - tauto.
+    - tauto.
+    - tauto.
+    - tauto.
+    - setoid_rewrite standardTruthDownSubstEq. eauto.
+    - setoid_rewrite standardTruthUpEq. firstorder.
+    - setoid_rewrite standardTruthUpEq. firstorder.
+    - setoid_rewrite standardTruthDownSubstEq. auto.
+    - congruence.
+    - congruence.
+    - congruence.
+    - congruence.
+    - congruence.
+    - congruence.
+    - intros [_ x] H. eapply n_Sn. eauto.
+    - firstorder.
+    - firstorder.
+    - firstorder.
+    - firstorder.
+    - firstorder.
+    - intros n A f H IH.
+      rewrite standardTruthDownSubstEq in H.
+      setoid_rewrite standardTruthLastSubstEq in IH.
       induction x as [ | x IHx].
       + exact H.
-      + specialize (IH x IHx). rewrite lastSubstitutionLemma in IH. exact IH.
+      + exact (IH x IHx).
   Qed.
 
+  (**
+  ** Notations
+  *)
+
   Module NOTATIONS.
-
     Delimit Scope HA with HA.
-
     Infix "﬩" := plus' (at level 64) : HA.
     Infix "⋅" := mult' (at level 63) : HA.
     Infix "≐" := atomEq (at level 65) : HA.
@@ -393,16 +434,18 @@ Module HA.
     Infix "→" := fImp (at level 69, right associativity) : HA.
     Notation "∃ A" := ∃A (at level 5) : HA.
     Notation "∀ A" := ∀A (at level 5) : HA.
-    Infix "//" := formulaSubstitution (at level 62, left associativity) : HA.
-    Infix "/+" := lastSubstitution (at level 62, left associativity) : HA.
-    Infix "/-" := downSubstitution (at level 62, left associativity) : HA.
+    Infix "//" := (fun A f => A//f) (at level 62, left associativity) : HA.
+    Infix "/+" := (fun A t => A/+t) (at level 62, left associativity) : HA.
+    Infix "/-" := (fun A t => A/-t) (at level 62, left associativity) : HA.
     Notation up := (fun A => up A).
-
   End NOTATIONS.
 
 End HA.
 
+(**
+** Coercions
+*)
+
 Module HA_COERCIONS.
-  Import HA.
-  Coercion fAtom : atom >-> formula.
+  Coercion HA.fAtom : HA.atom >-> HA.formula.
 End HA_COERCIONS.
