coq/pas.v
@@ -1,8 +1,13 @@
+(**
+* Partial applicative structures
+*)
+
 Require Import Coq.Classes.Morphisms.
 Require Import Coq.Classes.RelationClasses.
 Require Import Coq.Setoids.Setoid.
 
-Require Import myvec.
+Require Import fin.
+Require Import vec.
 
 Import FIN.NOTATIONS.
 Import VEC.NOTATIONS.
@@ -11,20 +16,23 @@ Local Open Scope VEC.
 
 Module PAS.
 
+  (**
+  ** Definition
+  For generality,
+  the carrier is a setoid and
+  application is a ternary relation that is
+  functional with respect to the setoid equality.
+  *)
+
   Local Reserved Infix "==" (at level 70).
   Class Pas := {
     carrier : Type;
-
     CarrierEq :
       carrier -> carrier -> Prop where "a == b" := (CarrierEq a b) : Pas;
-
     carrierEqEquivalence :> Equivalence CarrierEq;
-
     Appl : carrier -> carrier -> carrier -> Prop;
-
     applRespectful (a a' b b' c c' : carrier) :
       a == a' -> b == b' -> c == c' -> Appl a b c -> Appl a' b' c';
-
     applFunctional (a b c d : carrier) :  Appl a b c -> Appl a b d -> c == d
   }.
   Local Coercion carrier : Pas >-> Sortclass.
@@ -37,43 +45,47 @@ Module PAS.
     split; [ | symmetry in Ha, Hb, Hc]; eauto using applRespectful.
   Qed.
 
+  (**
+  ** Terms
+  *)
+
   Inductive term {pas : Pas} (n : nat) :=
-    termConst : pas -> term n
-  | termVar   : FIN.t n -> term n
-  | termConc  : term n -> term n -> term n.
-  Arguments termConst {_} {_} _.
-  Arguments termVar {_} {_} _.
-  Arguments termConc {_} {_} _ _.
-  Local Notation "& t" := (termConst t) (at level 6).
-  Local Infix "*" := termConc (at level 40, left associativity).
+  | const : pas -> term n
+  | var   : FIN.t n -> term n
+  | appl  : term n -> term n -> term n.
+  Arguments const {_} {_} _.
+  Arguments var {_} {_} _.
+  Arguments appl {_} {_} _ _.
+  Local Notation "& t" := (const t) (at level 6).
+  Local Infix "*" := appl (at level 40, left associativity).
 
-  Definition lastVar {_ : Pas} {n} : term (S n) := termVar FIN.last.
+  Definition lastVar {_ : Pas} {n} : term (S n) := var FIN.last.
 
-  Definition x11 {_ : Pas} : term 1 := termVar (FIN.ofNat 0 0).
-  Definition x12 {_ : Pas} : term 2 := termVar (FIN.ofNat 0 1).
-  Definition x22 {_ : Pas} : term 2 := termVar (FIN.ofNat 1 0).
-  Definition x13 {_ : Pas} : term 3 := termVar (FIN.ofNat 0 2).
-  Definition x23 {_ : Pas} : term 3 := termVar (FIN.ofNat 1 1).
-  Definition x33 {_ : Pas} : term 3 := termVar (FIN.ofNat 2 0).
-  Definition x14 {_ : Pas} : term 4 := termVar (FIN.ofNat 0 3).
-  Definition x24 {_ : Pas} : term 4 := termVar (FIN.ofNat 1 2).
-  Definition x34 {_ : Pas} : term 4 := termVar (FIN.ofNat 2 1).
-  Definition x44 {_ : Pas} : term 4 := termVar (FIN.ofNat 3 0).
-  Definition x15 {_ : Pas} : term 5 := termVar (FIN.ofNat 0 4).
-  Definition x25 {_ : Pas} : term 5 := termVar (FIN.ofNat 1 3).
-  Definition x35 {_ : Pas} : term 5 := termVar (FIN.ofNat 2 2).
-  Definition x45 {_ : Pas} : term 5 := termVar (FIN.ofNat 3 1).
-  Definition x55 {_ : Pas} : term 5 := termVar (FIN.ofNat 4 0).
+  Definition x01 {_ : Pas} : term 1 := var (FIN.ofNat 0 0).
+  Definition x02 {_ : Pas} : term 2 := var (FIN.ofNat 0 1).
+  Definition x12 {_ : Pas} : term 2 := var (FIN.ofNat 1 0).
+  Definition x03 {_ : Pas} : term 3 := var (FIN.ofNat 0 2).
+  Definition x13 {_ : Pas} : term 3 := var (FIN.ofNat 1 1).
+  Definition x23 {_ : Pas} : term 3 := var (FIN.ofNat 2 0).
+  Definition x04 {_ : Pas} : term 4 := var (FIN.ofNat 0 3).
+  Definition x14 {_ : Pas} : term 4 := var (FIN.ofNat 1 2).
+  Definition x24 {_ : Pas} : term 4 := var (FIN.ofNat 2 1).
+  Definition x34 {_ : Pas} : term 4 := var (FIN.ofNat 3 0).
+  Definition x05 {_ : Pas} : term 5 := var (FIN.ofNat 0 4).
+  Definition x15 {_ : Pas} : term 5 := var (FIN.ofNat 1 3).
+  Definition x25 {_ : Pas} : term 5 := var (FIN.ofNat 2 2).
+  Definition x35 {_ : Pas} : term 5 := var (FIN.ofNat 3 1).
+  Definition x45 {_ : Pas} : term 5 := var (FIN.ofNat 4 0).
 
   Fixpoint closedTermToTerm `{_ : Pas} {n} (t : term 0) : term n :=
   match t with
-  | &a        => &a
-  | termVar x => False_rect _ (FIN.t0Empty x)
-  | u*v       => closedTermToTerm u * closedTermToTerm v
+  | &a    => &a
+  | var x => False_rect _ (FIN.t0Empty x)
+  | u*v   => closedTermToTerm u * closedTermToTerm v
   end.
-  Local Notation "$ t" := (closedTermToTerm t) (at level 6).
+  Local Notation "§ t" := (closedTermToTerm t) (at level 6).
 
-  Lemma closedTermToTermLemma {_ : Pas} (t : term 0) : $ t = t.
+  Lemma closedTermToClosedTermEq {_ : Pas} (t : term 0) : §t = t.
   Proof.
     induction t as [a | x | u IHu v IHv]; simpl.
     - reflexivity.
@@ -81,38 +93,41 @@ Module PAS.
     - rewrite IHu, IHv. reflexivity.
   Qed.
 
+  (**
+  ** Vectors of terms
+  *)
+
   Definition pasVecToTermVec {pas : Pas} {m n : nat} (f : VEC.t pas n)
-    : VEC.t (term m) n := VEC.map termConst f.
+    : VEC.t (term m) n := VEC.map const f.
   Local Notation "&& P" := (pasVecToTermVec P) (at level 6).
 
-  Definition idVec {_ : Pas} {n} m : VEC.t (term (m + n)) n :=
-    VEC.finMap' termVar.
+  Definition idVec {_ : Pas} {n} k : VEC.t (term (k + n)) n := VEC.finMap' var.
+
+  (**
+  ** Substitution
+  *)
 
   Fixpoint substitution `{_ : Pas} {m n : nat} (t : term n)
                         (f : VEC.t (term m) n) : term m :=
   match t with
-  | &a        => &a
-  | termVar x => VEC.nth f x
-  | u*v       => substitution u f * substitution v f
+  | &a    => &a
+  | var x => VEC.nth f x
+  | u*v   => substitution u f * substitution v f
   end.
   Local Infix "/" := substitution.
 
-  Definition termVecSubst {_ : Pas} {n m k} (f : VEC.t (term m) n)
-                          (g : VEC.t (term k) m) : VEC.t (term k) n :=
-    VEC.map (fun t => t / g) f.
-
-  Lemma idVecSubstitution {pas : Pas} {n} (t : term n)
+  Lemma substIdVecEq {pas : Pas} {n} (t : term n)
     : t / idVec 0 = t.
   Proof.
     induction t as [a | x | u IHu v IHv].
     - reflexivity.
-    - unfold idVec, substitution. rewrite VEC.finMapNth'. reflexivity.
+    - unfold idVec, substitution. rewrite VEC.nthFinMapEq'. reflexivity.
     - simpl. setoid_rewrite IHu. setoid_rewrite IHv. reflexivity.
   Qed.
 
-  Lemma closedTermSubstitutionLemma {pas : Pas} {n m : nat} (t : term 0)
-                                    (f : VEC.t (term m) n) :
-    $ t / f = $ t.
+  Lemma closedTermSubstitutionEq {pas : Pas} {n m : nat} (t : term 0)
+                                 (f : VEC.t (term m) n) :
+    §t/f = §t.
   Proof.
     induction t as [a | x | u IHu v IHv]; simpl.
     - reflexivity.
@@ -120,42 +135,47 @@ Module PAS.
     - rewrite IHu, IHv. reflexivity.
   Qed.
 
-  Lemma closedTermSubstitutionLemma0 {pas : Pas} {n : nat} (t : term 0)
-                                     (f : VEC.t (term 0) n) :
-    $ t / f = t.
-  Proof. rewrite closedTermSubstitutionLemma. apply closedTermToTermLemma. Qed.
+  Lemma closedTermSubstitutionEq0 {pas : Pas} {n : nat} (t : term 0)
+                                  (f : VEC.t (term 0) n) :
+    §t/f = t.
+  Proof. rewrite closedTermSubstitutionEq. apply closedTermToClosedTermEq. Qed.
 
-  Lemma emptySubstitutionLemma {pas : Pas} {n} (t : term 0)
+  Lemma emptySubstitutionEq {pas : Pas} {n} (t : term 0)
                                (f : VEC.t (term n) 0) :
-    t / f = $ t.
+    t/f = §t.
   Proof.
-    rewrite <- closedTermToTermLemma at 1. apply closedTermSubstitutionLemma.
+    rewrite <- closedTermToClosedTermEq at 1. apply closedTermSubstitutionEq.
   Qed.
 
-  Lemma termVecIdSubstEq' {n m k} {pas : Pas} (f : VEC.t (term m) n)
-                          (g : VEC.t (term m) k) :
+  Definition termVecSubst {_ : Pas} {n m k} (f : VEC.t (term m) n)
+                          (g : VEC.t (term k) m) : VEC.t (term k) n :=
+    VEC.map (fun t => t/g) f.
+
+  Lemma termVecSubstIdVecEq {n m k} {pas : Pas} (f : VEC.t (term m) n)
+                            (g : VEC.t (term m) k) :
     termVecSubst (idVec k) (VEC.concat f g) = f.
   Proof.
     apply VEC.pointwiseEquality. intro x.
-    unfold termVecSubst. rewrite VEC.mapNth.
-    unfold idVec. rewrite VEC.finMapNth'.
+    unfold termVecSubst. rewrite VEC.nthMapEq.
+    unfold idVec. rewrite VEC.nthFinMapEq'.
     simpl.
     induction k as [ | k IHk].
     - reflexivity.
     - destruct g as [g t]. simpl. apply IHk.
   Qed.
 
+  (**
+  ** Product of a term and a vector of terms
+  *)
+
   Definition product {_ : Pas} {m n : nat} (t : term m) (f : VEC.t (term m) n)
-    : term m := VEC.foldL termConc t f.
+    : term m := VEC.foldl appl t f.
   Local Infix "**" := product (at level 39, left associativity).
 
-  Lemma emptyProductEq {pas : Pas} {n : nat} (t : term n) : t**() = t.
-  Proof. reflexivity. Qed.
-
-  Lemma productApplicationEq {pas : Pas} {n m k : nat} (t : term n)
-                             (f : VEC.t (term n) m) (g : VEC.t (term n) k) :
+  Lemma doubleProductEq {pas : Pas} {n m k : nat} (t : term n)
+                        (f : VEC.t (term n) m) (g : VEC.t (term n) k) :
     t ** f ** g = t ** (VEC.concat f g).
-  Proof. unfold product. rewrite VEC.concatFoldLEq. reflexivity. Qed.
+  Proof. unfold product. rewrite VEC.foldlConcatEq. reflexivity. Qed.
 
   Lemma productSubstitutionEq {pas : Pas} {n m k} (t : term m)
                               (f : VEC.t (term m) n) (g : VEC.t (term k) m) :
@@ -172,7 +192,7 @@ Module PAS.
                                    (f : VEC.t (term m) n)
                                    (g : VEC.t (term m) k) :
     (t ** idVec k) / VEC.concat f g = (t / VEC.concat f g) ** f.
-  Proof. rewrite productSubstitutionEq, termVecIdSubstEq'. reflexivity. Qed.
+  Proof. rewrite productSubstitutionEq, termVecSubstIdVecEq. reflexivity. Qed.
 
   Lemma idVecProductSubstitutionEq0 {pas : Pas} {n m} (t : term n)
                                     (f : VEC.t (term m) n) :
@@ -181,11 +201,11 @@ Module PAS.
 
   Lemma idVecProductSubstitutionEq0' {pas : Pas} {n} (t : term 0)
                                      (f : VEC.t (term 0) n) :
-    ($ t ** idVec 0) / f = t ** f.
+    (§t ** idVec 0) / f = t ** f.
   Proof.
     rewrite
       (idVecProductSubstitutionEq0 (n := n) (m := 0)),
-      closedTermSubstitutionLemma, closedTermToTermLemma.
+      closedTermSubstitutionEq, closedTermToClosedTermEq.
     reflexivity.
   Qed.
 
@@ -200,20 +220,25 @@ Module PAS.
 
   Lemma idVecProductSubstitutionEq1' {pas : Pas} {n} (u v : term 0)
                                      (f : VEC.t (term 0) n) :
-    ($ u ** idVec 1) / (f;; v) = u ** f.
+    (§u ** idVec 1) / (f;; v) = u ** f.
   Proof.
     assert ((f;; v) = VEC.concat f (();; v)) as H by reflexivity.
     setoid_rewrite H. clear H.
     rewrite
-      idVecProductSubstitutionEq, closedTermSubstitutionLemma,
-      closedTermToTermLemma.
+      idVecProductSubstitutionEq, closedTermSubstitutionEq,
+      closedTermToClosedTermEq.
     reflexivity.
   Qed.
 
-  Fixpoint Denotation `{pas : Pas} (t : term 0) (c : pas) : Prop := match t with
-  | &a        => a == c
-  | u*v       => exists a b, Denotation u a /\ Denotation v b /\ Appl a b c
-  | termVar _ => False
+  (**
+  ** Equivalence of closed terms
+  *)
+
+  Fixpoint Denotation `{pas : Pas} (t : term 0) (c : pas) : Prop :=
+  match t with
+  | &a    => a == c
+  | u*v   => exists a b, Denotation u a /\ Denotation v b /\ Appl a b c
+  | var _ => False
   end.
 
   Lemma denotationsUnique {pas : Pas} (t : term 0) (a b : pas) :
@@ -229,7 +254,7 @@ Module PAS.
       rewrite IHu, IHv in Habc. apply (applFunctional a' b'); assumption.
   Qed.
 
-  Definition ClosedTermEq {_ : Pas} (u v : term 0): Prop :=
+  Definition ClosedTermEq {_ : Pas} (u v : term 0) : Prop :=
     forall a, Denotation u a <-> Denotation v a.
   Local Infix "≃" := ClosedTermEq (at level 70).
 
@@ -269,18 +294,22 @@ Module PAS.
         rewrite <- Ha. exact H.
   Qed.
 
-  Instance termConstProper {pas : Pas} :
-    Proper (CarrierEq ==> ClosedTermEq) termConst.
+  (**
+  *** Correctness properties
+  *)
+
+  Instance constProper {pas : Pas} :
+    Proper (CarrierEq ==> ClosedTermEq) const.
   Proof. intros a b Hab c. simpl. rewrite Hab. tauto. Qed.
 
-  Instance termConcProper {pas : Pas} :
-    Proper (ClosedTermEq ==> ClosedTermEq ==> ClosedTermEq) termConc.
+  Instance applProper' {pas : Pas} :
+    Proper (ClosedTermEq ==> ClosedTermEq ==> ClosedTermEq) appl.
   Proof.
     intros u u' Hu v v' Hv c. simpl. setoid_rewrite Hu. setoid_rewrite Hv.
     tauto.
   Qed.
 
-  Lemma termConstInjective {pas : Pas} (a b : pas) : &a ≃ &b -> a == b.
+  Lemma constInjective {pas : Pas} (a b : pas) : &a ≃ &b -> a == b.
   Proof. intro H. specialize (H b). simpl in H. apply H. reflexivity. Qed.
 
   Lemma correctness1 {pas : Pas} (u v : term 0) (c : pas) :
@@ -303,7 +332,7 @@ Module PAS.
   Proof.
     rewrite correctness1. split.
     - intros [a' [b' [Ha [Hb H]]]].
-      apply termConstInjective in Ha. apply termConstInjective in Hb.
+      apply constInjective in Ha. apply constInjective in Hb.
       rewrite Ha, Hb. exact H.
     - intro H. exists a, b. firstorder.
   Qed.
@@ -318,6 +347,10 @@ Module PAS.
 
   Global Opaque Denotation ClosedTermEq.
 
+  (**
+  ** Denoting closed terms
+  *)
+
   Definition Denotes {pas : Pas} (t : term 0) : Prop := exists a : pas, t ≃ &a.
   Hint Unfold Denotes.
   Local Notation "t !" := (Denotes t) (at level 70).
@@ -325,17 +358,24 @@ Module PAS.
   Instance denotesProper {pas : Pas} : Proper (ClosedTermEq ==> iff) Denotes.
   Proof. intros u v H. unfold Denotes. setoid_rewrite H. tauto. Qed.
 
-  Inductive SubTerm {pas : Pas} {n} : term n -> term n -> Prop :=
-  | subTermRefl u     : SubTerm u u
-  | subTermL    u v w : SubTerm u v -> SubTerm u (v*w)
-  | subTermR    u v w : SubTerm u w -> SubTerm u (v*w).
-  Hint Constructors SubTerm.
+  (**
+  ** Subterms
+  *)
 
-  Instance subTermReflexive {pas : Pas} {n} : Reflexive (SubTerm (n := n)).
+  Inductive Subterm {pas : Pas} {n} : term n -> term n -> Prop :=
+  | subtermRefl u     : Subterm u u
+  | subtermL    u v w : Subterm u v -> Subterm u (v*w)
+  | subtermR    u v w : Subterm u w -> Subterm u (v*w).
+  Hint Constructors Subterm.
+
+  Instance subtermReflexive {pas : Pas} {n} : Reflexive (Subterm (n := n)).
   Proof. auto. Qed.
 
-  Lemma subTermDenotes {pas : Pas} (u v : term 0) :
-    SubTerm u v -> v! -> u!.
+  Instance subtermTransitive {pas : Pas} {n} : Transitive (Subterm (n := n)).
+  Proof. intros u v w Huv Hvw. induction Hvw; auto. Qed.
+
+  Lemma subtermDenotes {pas : Pas} (u v : term 0) :
+    Subterm u v -> v! -> u!.
   Proof.
     intros H. induction H as [ | u v w H IH | u v w H IH].
     - tauto.
@@ -343,36 +383,40 @@ Module PAS.
     - unfold Denotes. setoid_rewrite correctness1. firstorder.
   Qed.
 
-  Lemma subTermDenotesProduct {pas : Pas} {n : nat} (t : term 0)
+  Lemma subtermDenotesProduct {pas : Pas} {n : nat} (t : term 0)
                               (f : VEC.t (term 0) n) :
     t**f! -> t!.
   Proof.
     induction n as [ | n IHn].
     - destruct f. tauto.
     - destruct f as [f a]. intro H. apply (IHn f).
-      apply subTermDenotes with (v := (t ** (f;; a))); [ | exact H].
-      apply subTermL. reflexivity.
+      apply subtermDenotes with (v := (t ** (f;; a))); [ | exact H].
+      apply subtermL. reflexivity.
   Qed.
 
+  (**
+  ** Notations
+  *)
+
   Module NOTATIONS.
-
     Delimit Scope PAS with PAS.
-
-    Notation "$ t" := $ t (at level 6) : PAS.
+    Notation "§ t" := § t (at level 6) : PAS.
     Notation "& t" := &t (at level 6) : PAS.
     Notation "&& f" := &&f (at level 6) : PAS.
     Notation "t !" := (t!) (at level 70) : PAS.
-    Infix "*" := termConc : PAS.
+    Infix "*" := appl : PAS.
     Infix "**" := product (at level 39, left associativity) : PAS.
     Infix "/" := substitution : PAS.
     Infix "==" := CarrierEq (at level 70) : PAS.
     Infix "≃" := ClosedTermEq (at level 70) : PAS.
-
   End NOTATIONS.
 
 End PAS.
 
+(**
+** Coercions
+*)
+
 Module PAS_COERCIONS.
-  Import PAS.
-  Coercion carrier : Pas >-> Sortclass.
+  Coercion PAS.carrier : PAS.Pas >-> Sortclass.
 End PAS_COERCIONS.
