coq/pcarealizability.v
@@ -1,9 +1,14 @@
+(**
+* Realizability with partial combinatory algebras
+*)
+
 Require Import Coq.Classes.Morphisms.
 
+Require Import fin.
 Require Import heytingarithmetic.
-Require Import myvec.
 Require Import pas.
 Require Import pca.
+Require Import vec.
 
 Import FIN.NOTATIONS.
 Import HA.NOTATIONS.
@@ -23,14 +28,18 @@ Local Open Scope PCA.
 Local Notation Pca := PCA.Pca.
 Local Notation k := PCA.k.
 Local Notation s := PCA.s.
-Local Notation x11 := PAS.x11.
+Local Notation x01 := PAS.x01.
+Local Notation x02 := PAS.x02.
 Local Notation x12 := PAS.x12.
-Local Notation x22 := PAS.x22.
+Local Notation x03 := PAS.x03.
 Local Notation x13 := PAS.x13.
 Local Notation x23 := PAS.x23.
-Local Notation x33 := PAS.x33.
 
 Module PCA_REL.
+
+  (**
+  ** Definition
+  *)
 
   Local Notation "## f" :=
     (VEC.map (fun x => #x) f) (at level 6, right associativity).
@@ -56,6 +65,9 @@ Module PCA_REL.
       fun f t => exists n : nat, π1*t ≃ #n /\ Realizability P (f, n) (π2*t)
   | ∀P         => fun f t => forall x : nat, Realizability P (f, x) (t*#x)
   end.
+
+  Definition IsRealizable {_ : Pca} {n} (P : HA.formula n) : Prop :=
+    exists t : PAS.term 0, forall f : VEC.t nat n, Realizability P f (t**##f).
 
   Lemma realizabilityRespectful {pca : Pca} {n} (A : HA.formula n)
                                 (f : VEC.t nat n) (u v : PAS.term 0) :
@@ -111,83 +123,86 @@ Module PCA_REL.
       [n A | n A IHA B _ | n A IHA B IHB | n A _ B _ | n A IH | n A IH];
     simpl; intro t.
     - unfold AtomicRealizability. tauto.
-    - intros [H _]. eauto using PAS.subTermDenotes.
-    - intros [ [H H'] | [H H'] ]; eauto using PAS.subTermDenotes.
+    - intros [H _]. eauto using PAS.subtermDenotes.
+    - intros [ [H H'] | [H H'] ]; eauto using PAS.subtermDenotes.
     - tauto.
-    - intros [x [H H'] ]. eauto using PAS.subTermDenotes.
-    - intros H. specialize (H 0). eauto using PAS.subTermDenotes.
+    - intros [x [H H'] ]. eauto using PAS.subtermDenotes.
+    - intros H. specialize (H 0). eauto using PAS.subtermDenotes.
   Qed.
 
-  Lemma substitutionLemma {pca : Pca} {n m} (A : HA.formula n)
-                          (f : VEC.t (HA.term m) n) (g : VEC.t nat m)
-                          (t : PAS.term 0) :
-    Realizability (A // f) g t <->
-    Realizability  A (HA.vecStandardValuation f g) t.
+  (**
+  ** Realizability and substitution
+  *)
+
+  Lemma realizabilitySubstitution {pca : Pca} {n m} (A : HA.formula n)
+                                  (f : VEC.t (HA.term m) n) (g : VEC.t nat m)
+                                  (t : PAS.term 0) :
+    Realizability (A // f) g t <-> Realizability  A (HA.standardVecVal f g) t.
   Proof.
     generalize dependent m. generalize dependent t.
     induction A as
       [n A | n A IHA B IHB | n A IHA B IHB | n A IHA B IHB | n A IH | n A IH];
     intros m f g; simpl.
     - unfold AtomicRealizability.
-      setoid_rewrite HA.atomSubstitutionLemma.
+      setoid_rewrite HA.atomicTruthSubstEq.
       tauto.
     - setoid_rewrite IHA. setoid_rewrite IHB. tauto.
     - setoid_rewrite IHA. setoid_rewrite IHB. tauto.
     - setoid_rewrite IHA. setoid_rewrite IHB. tauto.
-    - setoid_rewrite IH. setoid_rewrite HA.termVecUpValuationLemma'. tauto.
-    - setoid_rewrite IH. setoid_rewrite HA.termVecUpValuationLemma'. tauto.
+    - setoid_rewrite IH. setoid_rewrite HA.standardVecValTermVecUpEq'. tauto.
+    - setoid_rewrite IH. setoid_rewrite HA.standardVecValTermVecUpEq'. tauto.
   Qed.
 
-  Lemma lastSubstitutionLemma {pca : Pca} {n} (A : HA.formula (S n))
-                              (t : HA.term (S n)) (f : VEC.t nat n) (x : nat)
-                              (u : PAS.term 0) :
+  Lemma realizabilityLastSubstitution {pca : Pca} {n} (A : HA.formula (S n))
+                                      (t : HA.term (S n)) (f : VEC.t nat n)
+                                      (x : nat) (u : PAS.term 0) :
     Realizability (A /+ t) (f, x) u <->
-    Realizability A (f, HA.standardValuation t (f, x)) u.
+    Realizability A (f, HA.standardVal t (f, x)) u.
   Proof.
-    setoid_rewrite substitutionLemma.
+    setoid_rewrite realizabilitySubstitution.
     assert
-      (HA.vecStandardValuation (HA.idVecUp;; t) (f;; x) =
-       (HA.vecStandardValuation HA.idVecUp (f;; x));;
-        HA.standardValuation t (f;; x))
+      (HA.standardVecVal (HA.idVecUp;; t) (f;; x) =
+       (HA.standardVecVal HA.idVecUp (f;; x));; HA.standardVal t (f;; x))
     as H by reflexivity.
     rewrite H. clear H.
-    setoid_rewrite HA.idVecUpValuationLemma.
+    setoid_rewrite HA.standardVecValIdVecUpEq.
     tauto.
   Qed.
 
-  Lemma downSubstitutionLemma {pca : Pca} {n} (A : HA.formula (S n))
-                              (t : HA.term n) (f : VEC.t nat n)
-                              (u : PAS.term 0) :
-    Realizability (A /- t) f u <->
-    Realizability A (f, HA.standardValuation t f) u.
+  Lemma realizabilityDownSubstitution {pca : Pca} {n} (A : HA.formula (S n))
+                                      (t : HA.term n) (f : VEC.t nat n)
+                                      (u : PAS.term 0) :
+    Realizability (A /- t) f u <-> Realizability A (f, HA.standardVal t f) u.
   Proof.
-    setoid_rewrite substitutionLemma.
+    setoid_rewrite realizabilitySubstitution.
     assert
-      (HA.vecStandardValuation (HA.idVec;; t) f =
-       (HA.vecStandardValuation HA.idVec f);; HA.standardValuation t f)
+      (HA.standardVecVal (HA.idVec;; t) f =
+       (HA.standardVecVal HA.idVec f);; HA.standardVal t f)
     as H by reflexivity.
     rewrite H. clear H.
-    setoid_rewrite HA.idVecValuationLemma.
+    setoid_rewrite HA.standardVecValIdVecEq.
     tauto.
   Qed.
 
-  Lemma upLemma {pca : Pca} {n} (A : HA.formula n) (f : VEC.t nat n) (x : nat)
-                (t : PAS.term 0) :
+  Lemma realizabilityUp {pca : Pca} {n} (A : HA.formula n) (f : VEC.t nat n)
+                        (x : nat) (t : PAS.term 0) :
     Realizability (up A) (f, x) t <-> Realizability A f t.
   Proof.
-    unfold HA.formulaUp. rewrite substitutionLemma, HA.idVecUpValuationLemma.
+    unfold HA.formulaUp.
+    rewrite realizabilitySubstitution, HA.standardVecValIdVecUpEq.
     tauto.
   Qed.
 
-  Definition IsRealizable {_ : Pca} {n} (P : HA.formula n) : Prop :=
-    exists t : PAS.term 0, forall f : VEC.t nat n, Realizability P f (t**##f).
+  (**
+  ** Combinatory completeness for products of natural representations
+  *)
 
   Lemma combinatoryCompleteness1 {pca : Pca} {n} (t : PAS.term (S n))
                                  (f : VEC.t nat n) :
     λ t ** ##f!.
   Proof.
     apply PCA.combinatoryCompleteness1'.
-    intro x. rewrite VEC.mapNth. apply PCA.natRepresentationCombinatorDenotes.
+    intro x. rewrite VEC.nthMapEq. apply PCA.natRepresentationCombinatorDenotes.
   Qed.
 
   Lemma combinatoryCompleteness2 {pca : Pca} {n} (t : PAS.term n)
@@ -195,7 +210,7 @@ Module PCA_REL.
     λ t ** ##f ≃ t/##f.
   Proof.
     apply PCA.combinatoryCompleteness2'.
-    intro x. rewrite VEC.mapNth. apply PCA.natRepresentationCombinatorDenotes.
+    intro x. rewrite VEC.nthMapEq. apply PCA.natRepresentationCombinatorDenotes.
   Qed.
 
   Lemma combinatoryCompleteness2' {pca : Pca} {n} (t : PAS.term (S n))
@@ -205,57 +220,64 @@ Module PCA_REL.
     cutrewrite (λ t ** ##f * &a = λ t ** (##f;; &a)); [ | reflexivity].
     apply PCA.combinatoryCompleteness2'.
     destruct x as [x | x]; simpl.
-    - rewrite VEC.mapNth. apply PCA.natRepresentationCombinatorDenotes.
+    - rewrite VEC.nthMapEq. apply PCA.natRepresentationCombinatorDenotes.
     - exists a. reflexivity.
   Qed.
 
-  Fixpoint termRepresentation {pca : Pca} {n} (t : HA.term n) : PAS.term 0 :=
-  match t with
-  | HA.O'       => λ (n := n) $ #0
-  | HA.var x    => λ (PAS.termVar x)
-  | HA.S' t     => λ (n := n) ($ σ * $ (termRepresentation t) ** PAS.idVec 0)
-  | u ﬩ v       =>
-    let u' := $ (termRepresentation u) ** PAS.idVec 0 in
-    let v' := $ (termRepresentation v) ** PAS.idVec 0 in
-    λ (n := n) ($ α * u' * v')
-  | u ⋅ v       =>
-    let u' := $ (termRepresentation u) ** PAS.idVec 0 in
-    let v' := $ (termRepresentation v) ** PAS.idVec 0 in
-    λ (n := n) ($ μ * u' * v')
-  end.
-  Local Notation termRep := termRepresentation.
+  (**
+  ** Term representation
+  *)
 
-  Lemma termRepresentationCorrect {pca : Pca} {n} (t : HA.term n)
-                                  (f : VEC.t nat n) :
-    (termRep t)**##f ≃ #(HA.standardValuation t f).
+  Fixpoint termRep {pca : Pca} {n} (t : HA.term n) : PAS.term 0 :=
+  match t with
+  | HA.O'       => λ (n := n) §#0
+  | HA.var x    => λ (PAS.var x)
+  | HA.S' t     => λ (n := n) (§σ * §(termRep t) ** PAS.idVec 0)
+  | u ﬩ v       =>
+    let u' := §(termRep u) ** PAS.idVec 0 in
+    let v' := §(termRep v) ** PAS.idVec 0 in
+    λ (n := n) (§α * u' * v')
+  | u ⋅ v       =>
+    let u' := §(termRep u) ** PAS.idVec 0 in
+    let v' := §(termRep v) ** PAS.idVec 0 in
+    λ (n := n) (§μ * u' * v')
+  end.
+
+  Lemma termRepCorrect {pca : Pca} {n} (t : HA.term n) (f : VEC.t nat n) :
+    (termRep t)**##f ≃ #(HA.standardVal t f).
   Proof.
     induction t as [ | x | t IHt | u IHu v IHv | u IHu v IHv];
     simpl; rewrite combinatoryCompleteness2; simpl.
-    - setoid_rewrite PAS.closedTermSubstitutionLemma0. reflexivity.
-    - rewrite VEC.mapNth. reflexivity.
+    - setoid_rewrite PAS.closedTermSubstitutionEq0. reflexivity.
+    - rewrite VEC.nthMapEq. reflexivity.
     - setoid_rewrite PAS.idVecProductSubstitutionEq0'.
-      setoid_rewrite PAS.closedTermSubstitutionLemma0.
+      setoid_rewrite PAS.closedTermSubstitutionEq0.
       rewrite IHt.
       rewrite PCA.successorCombinatorCorrect.
       reflexivity.
     - setoid_rewrite PAS.idVecProductSubstitutionEq0'.
-      setoid_rewrite PAS.closedTermSubstitutionLemma0.
+      setoid_rewrite PAS.closedTermSubstitutionEq0.
       rewrite IHu, IHv.
       rewrite PCA.additionCombinatorCorrect.
       reflexivity.
     - setoid_rewrite PAS.idVecProductSubstitutionEq0'.
-      setoid_rewrite PAS.closedTermSubstitutionLemma0.
+      setoid_rewrite PAS.closedTermSubstitutionEq0.
       rewrite IHu, IHv.
       rewrite PCA.multiplicationCombinatorCorrect.
       reflexivity.
   Qed.
 
-  Instance realizabilityModel {pca : Pca} : HA.Model (@IsRealizable _).
+  (**
+  ** The realizability interpretation
+  *)
+
+  Instance realizabilityInterpretation {pca : Pca} :
+    HA.Interpretation (@IsRealizable _).
   Proof.
     split.
     - intros [t H]. specialize (H ()). destruct H as [H _]. exact H.
     - intros n A B [u Hu] [v Hv].
-      exists (λ (n := n) ($ u ** PAS.idVec 0 * $ v ** PAS.idVec 0)).
+      exists (λ (n := n) (§u ** PAS.idVec 0 * §v ** PAS.idVec 0)).
       intro f.
       specialize (Hu f). specialize (Hv f).
       rewrite combinatoryCompleteness2.
@@ -264,9 +286,9 @@ Module PCA_REL.
       destruct Hu as [_ Hu]. exact (Hu _ Hv).
     - intros n A [t H]. exists t. intro f. simpl. intro x. apply H.
     - intros n A [t H].
-      exists (λ (n := (S n)) ($ t ** PAS.idVec 1)).
+      exists (λ (n := (S n)) (§t ** PAS.idVec 1)).
       intros [f x].
-      rewrite combinatoryCompleteness2, upLemma.
+      rewrite combinatoryCompleteness2, realizabilityUp.
       assert (##(f;; x) = (##f;; #x)) as H' by reflexivity.
       rewrite H'. clear H'.
       setoid_rewrite PAS.idVecProductSubstitutionEq1'.
@@ -298,9 +320,9 @@ Module PCA_REL.
       destruct Ha as [_ Ha], Hb as [_ Hb].
       specialize (Ha _ Hc). specialize (Hb _ Hc).
       destruct Ha as [_ Ha]. exact (Ha _ Hb).
-    - intros n A B. exists (λ (n := n) $ π). intro f.
+    - intros n A B. exists (λ (n := n) §π). intro f.
       rewrite combinatoryCompleteness2.
-      setoid_rewrite PAS.closedTermSubstitutionLemma0.
+      setoid_rewrite PAS.closedTermSubstitutionEq0.
       split; [ apply PCA.pairingCombinatorDenotes | ].
       intros t Ha. destruct (realizersDenote Ha) as [a Ht]. rewrite Ht in *.
       clear dependent t.
@@ -310,17 +332,17 @@ Module PCA_REL.
       split.
       + rewrite PCA.leftProjectionCombinatorCorrect. exact Ha.
       + rewrite PCA.rightProjectionCombinatorCorrect. exact Hb.
-    - intros n A B. exists (λ (n := n) $ π1). intro f.
+    - intros n A B. exists (λ (n := n) §π1). intro f.
       rewrite combinatoryCompleteness2.
-      setoid_rewrite PAS.closedTermSubstitutionLemma0.
+      setoid_rewrite PAS.closedTermSubstitutionEq0.
       split; [apply PCA.leftProjectionCombinatorDenotes | ]. simpl. tauto.
-    - intros n A B. exists (λ (n := n) $ π2). intro f.
+    - intros n A B. exists (λ (n := n) §π2). intro f.
       rewrite combinatoryCompleteness2.
-      setoid_rewrite PAS.closedTermSubstitutionLemma0.
+      setoid_rewrite PAS.closedTermSubstitutionEq0.
       split; [apply PCA.rightProjectionCombinatorDenotes | ]. simpl. tauto.
-    - intros n A B. exists (λ (n := n) ($ (π * #0))). intro f.
+    - intros n A B. exists (λ (n := n) (§(π * #0))). intro f.
       rewrite combinatoryCompleteness2.
-      setoid_rewrite PAS.closedTermSubstitutionLemma0.
+      setoid_rewrite PAS.closedTermSubstitutionEq0.
       destruct (PCA.natRepresentationCombinatorDenotes 0) as [x Hx].
       rewrite Hx.
       split; [apply PCA.pairingCombinatorDenotes' | ].
@@ -329,9 +351,9 @@ Module PCA_REL.
       left. split.
       + rewrite PCA.leftProjectionCombinatorCorrect, Hx. reflexivity.
       + rewrite PCA.rightProjectionCombinatorCorrect. exact Ha.
-    - intros n A B. exists (λ (n := n) ($ (π * #1))). intro f.
+    - intros n A B. exists (λ (n := n) (§(π * #1))). intro f.
       rewrite combinatoryCompleteness2.
-      setoid_rewrite PAS.closedTermSubstitutionLemma0.
+      setoid_rewrite PAS.closedTermSubstitutionEq0.
       destruct (PCA.natRepresentationCombinatorDenotes 1) as [x Hx].
       rewrite Hx.
       split; [apply PCA.pairingCombinatorDenotes' | ].
@@ -341,15 +363,15 @@ Module PCA_REL.
       + rewrite PCA.leftProjectionCombinatorCorrect, Hx. reflexivity.
       + rewrite PCA.rightProjectionCombinatorCorrect. exact Ha.
     - intros n A B C.
-      set (t := $ δ * x23 * x33 * ($ π1 * x13) * ($ π2 * x13)). simpl in t.
-      exists (λ (n := n) $ (λ t)). intro f.
+      set (t := §δ * x13 * x23 * (§π1 * x03) * (§π2 * x03)). simpl in t.
+      exists (λ (n := n) §(λ t)). intro f.
       rewrite combinatoryCompleteness2.
-      setoid_rewrite PAS.closedTermSubstitutionLemma0.
+      setoid_rewrite PAS.closedTermSubstitutionEq0.
       split; [apply PCA.representationsDenote | ].
       intros u Ha. destruct (realizersDenote Ha) as [a Hu]. rewrite Hu in *.
       clear dependent u.
       split. {
-        apply PAS.subTermDenotes with (v := λ t * &a * &a); [auto | ].
+        apply PAS.subtermDenotes with (v := λ t * &a * &a); [auto | ].
         cutrewrite (λ t * &a * &a = λ t ** &&(();; a;; a)); [ | reflexivity].
         apply PCA.combinatoryCompleteness1.
       }
@@ -362,7 +384,7 @@ Module PCA_REL.
       intros u Hc. destruct (realizersDenote Hc) as [c Hu]. rewrite Hu in *.
       clear dependent u.
       rewrite PCA.combinatoryCompletenessInstance3. simpl.
-      setoid_rewrite PAS.closedTermSubstitutionLemma0.
+      setoid_rewrite PAS.closedTermSubstitutionEq0.
       destruct Ha as [[H H'] | [H H']]; rewrite H.
       + setoid_rewrite PCA.caseCombinatorCorrect0.
         destruct Hb as [_ Hb]. exact (Hb _ H').
@@ -372,27 +394,27 @@ Module PCA_REL.
       rewrite combinatoryCompleteness2. simpl.
       split; [exists k; reflexivity | ]. intros v [H _]. contradiction.
     - intros n A t.
-      exists (λ (n := S n) ($ π * $ (termRep t) ** PAS.idVec 1 * PAS.lastVar)).
+      exists (λ (n := S n) (§π * §(termRep t) ** PAS.idVec 1 * PAS.lastVar)).
       intro f.
       split; [apply combinatoryCompleteness1 | ].
       intros u Ha. destruct (realizersDenote Ha) as [a Hu]. rewrite Hu in *.
       clear dependent u.
-      rewrite downSubstitutionLemma in Ha.
-      set (x := HA.standardValuation t f). exists x.
+      rewrite realizabilityDownSubstitution in Ha.
+      set (x := HA.standardVal t f). exists x.
       rewrite combinatoryCompleteness2'. simpl.
-      setoid_rewrite PAS.closedTermSubstitutionLemma0.
+      setoid_rewrite PAS.closedTermSubstitutionEq0.
       setoid_rewrite PAS.idVecProductSubstitutionEq1'.
-      rewrite termRepresentationCorrect. fold x. fold x in Ha.
+      rewrite termRepCorrect. fold x. fold x in Ha.
       destruct (PCA.natRepresentationCombinatorDenotes x) as [x' Hx].
       rewrite Hx.
       split.
       + apply PCA.leftProjectionCombinatorCorrect.
       + setoid_rewrite PCA.rightProjectionCombinatorCorrect. exact Ha.
     - intros n A B.
-      set (t := λ (x12 * ($ π1 * x22) * ($ π2 * x22))).
-      exists (λ (n := n) $ t). intro f.
+      set (t := λ (x02 * (§π1 * x12) * (§π2 * x12))).
+      exists (λ (n := n) §t). intro f.
       rewrite combinatoryCompleteness2.
-      setoid_rewrite PAS.closedTermSubstitutionLemma0.
+      setoid_rewrite PAS.closedTermSubstitutionEq0.
       split; [ apply PCA.representationsDenote | ].
       intros u Ha. destruct (realizersDenote Ha) as [a Hu]. rewrite Hu in *.
       clear dependent u.
@@ -403,20 +425,20 @@ Module PCA_REL.
       intros u Hb. destruct (realizersDenote Hb) as [b Hu]. rewrite Hu in *.
       clear dependent u.
       unfold t. rewrite PCA.combinatoryCompletenessInstance2. simpl.
-      setoid_rewrite PAS.closedTermSubstitutionLemma0.
+      setoid_rewrite PAS.closedTermSubstitutionEq0.
       destruct Hb as [x [Hx Hb]]. rewrite Hx in *.
       simpl in Ha. specialize (Ha x). destruct Ha as [_ Ha].
-      specialize (Ha _ Hb). apply upLemma in Ha. exact Ha.
+      specialize (Ha _ Hb). apply realizabilityUp in Ha. exact Ha.
     - intros n A B.
-      set (t := λ (x13*x33*x23)).
-      exists (λ (n := n) $ t). intro f.
+      set (t := λ (x03*x23*x13)).
+      exists (λ (n := n) §t). intro f.
       rewrite combinatoryCompleteness2.
-      setoid_rewrite PAS.closedTermSubstitutionLemma0.
+      setoid_rewrite PAS.closedTermSubstitutionEq0.
       split; [apply PCA.representationsDenote | ].
       intros u Ha. destruct (realizersDenote Ha) as [a Hu]. rewrite Hu in *.
       clear dependent u.
       split. {
-        apply PAS.subTermDenotes with (v := t*&a*&a); [auto | ].
+        apply PAS.subtermDenotes with (v := t*&a*&a); [auto | ].
         cutrewrite (t * &a * &a  = t ** &&(();; a;; a)); [ | reflexivity].
         apply PCA.combinatoryCompleteness1.
       }
@@ -427,16 +449,16 @@ Module PCA_REL.
       rewrite Hx in *.
       unfold t. rewrite PCA.combinatoryCompletenessInstance3. simpl.
       simpl in Ha. specialize (Ha x). destruct Ha as [_ Ha].
-      setoid_rewrite upLemma in Ha.
+      setoid_rewrite realizabilityUp in Ha.
       rewrite <- Hx. exact (Ha _ Hb).
     - intros n A t.
-      exists (λ (n := S n) (PAS.lastVar * $ (termRep t) ** PAS.idVec 1)).
+      exists (λ (n := S n) (PAS.lastVar * §(termRep t) ** PAS.idVec 1)).
       split; [apply combinatoryCompleteness1 | ].
       intros u Ha. destruct (realizersDenote Ha) as [a Hu]. rewrite Hu in *.
       clear dependent u.
-      rewrite downSubstitutionLemma, combinatoryCompleteness2'. simpl.
+      rewrite realizabilityDownSubstitution, combinatoryCompleteness2'. simpl.
       setoid_rewrite PAS.idVecProductSubstitutionEq1'.
-      rewrite termRepresentationCorrect.
+      rewrite termRepCorrect.
       apply Ha.
     - exists (λ (n := 1) &k).
       intros [f x]. destruct f.
@@ -488,7 +510,7 @@ Module PCA_REL.
       intros [f x]. destruct f.
       rewrite combinatoryCompleteness2.
       split; [exists k; reflexivity | ].
-      intros u [Ha _]. simpl in Ha. exfalso. intuition.
+      intros u [Ha _]. simpl in Ha. exfalso. eapply n_Sn. eauto.
     - exists (λ (n := 2) &k).
       intros [[f x] y]. destruct f.
       rewrite combinatoryCompleteness2.
@@ -517,15 +539,15 @@ Module PCA_REL.
       split; [ | exists k; reflexivity].
       simpl. auto.
     - intros n A.
-      set (t := λ ($ ρ * x13 * x23 * x33)).
-      exists (λ (n := n) $ t). intro f.
+      set (t := λ (§ρ * x03 * x13 * x23)).
+      exists (λ (n := n) §t). intro f.
       rewrite combinatoryCompleteness2.
-      setoid_rewrite PAS.closedTermSubstitutionLemma0.
+      setoid_rewrite PAS.closedTermSubstitutionEq0.
       split; [ apply PCA.representationsDenote | ].
       intros u Ha. destruct (realizersDenote Ha) as [a Hu]. rewrite Hu in *.
       clear dependent u.
       split. {
-        apply PAS.subTermDenotes with (v := t*&a*&a); [auto | ].
+        apply PAS.subtermDenotes with (v := t*&a*&a); [auto | ].
         cutrewrite (t * &a * &a  = t ** &&(();; a;; a)); [ | reflexivity].
         apply PCA.combinatoryCompleteness1.
       }
@@ -535,17 +557,21 @@ Module PCA_REL.
       destruct (PCA.natRepresentationCombinatorDenotes x) as [x' Hx].
       rewrite Hx in *.
       unfold t. rewrite PCA.combinatoryCompletenessInstance3. simpl.
-      setoid_rewrite PAS.closedTermSubstitutionLemma0. rewrite <- Hx.
+      setoid_rewrite PAS.closedTermSubstitutionEq0. rewrite <- Hx.
       clear dependent x'.
       induction x as [ | x IHx].
       + setoid_rewrite PCA.primitiveRecursionCombinatorCorrect0.
-        rewrite downSubstitutionLemma in Ha. exact Ha.
+        rewrite realizabilityDownSubstitution in Ha. exact Ha.
       + setoid_rewrite PCA.primitiveRecursionCombinatorCorrectS.
         destruct (realizersDenote IHx) as [c Hc]. rewrite Hc in *.
         simpl in Hb. specialize (Hb x). destruct Hb as [_ Hb].
         specialize (Hb _ IHx).
-        setoid_rewrite lastSubstitutionLemma in Hb. exact Hb.
+        setoid_rewrite realizabilityLastSubstitution in Hb. exact Hb.
   Qed.
+
+  (**
+  ** Notations
+  *)
 
   Module NOTATIONS.
 
