coq/termpca.v
@@ -1,9 +1,13 @@
+(**
+* A term partial combinatory algebra
+*)
+
 Require Import Coq.Classes.Morphisms.
 Require Import Coq.Classes.RelationClasses.
 Require Import Coq.Relations.Relations.
 Require Import Coq.Relations.Relation_Operators.
 
-Require Import myvec.
+Require Import fin.
 Require Import pas.
 Require Import pca.
 Require Import relationresults.
@@ -16,65 +20,84 @@ Import REL_RES.NOTATIONS.
 
 Local Open Scope REL_RES.
 
+Ltac inj_subst H := injection H; intros; subst; clear H.
+
 Module TERM_PCA.
 
+  (**
+  ** Terms
+  *)
+
   Inductive term : Type :=
-    K    : term
+  | K    : term
   | S    : term
-  | conc : term -> term -> term.
-  Local Infix "⋅" := conc (at level 40, left associativity).
+  | appl : term -> term -> term.
+  Local Infix "⋅" := appl (at level 40, left associativity).
 
-  (* one step reduction relation *)
+  (**
+  ** One step reduction relation
+  *)
+
+  Local Reserved Infix ">" (at level 70).
   Inductive OneStepRed : relation term :=
-    oneStepRedK u v    : OneStepRed (K⋅u⋅v) u
-  | oneStepRedS u v w  : OneStepRed (S⋅u⋅v⋅w) (u⋅w⋅(v⋅w))
-  | oneStepRedL u u' v : OneStepRed u u' -> OneStepRed (u⋅v) (u'⋅v)
-  | oneStepRedR u v v' : OneStepRed v v' -> OneStepRed (u⋅v) (u⋅v').
-  Local Infix ">" := OneStepRed (at level 70).
+  | oneStepRedK u v    : K⋅u⋅v > u
+  | oneStepRedS u v w  : S⋅u⋅v⋅w > u⋅w⋅(v⋅w)
+  | oneStepRedL u u' v : u > u' -> u⋅v > u'⋅v
+  | oneStepRedR u v v' : v > v' -> u⋅v > u⋅v'
+  where "u > v" := (OneStepRed u v).
 
-  (* reduction relation *)
+  (**
+  ** Reduction relation
+  *)
+
   Definition Red := OneStepRed+.
   Local Infix ">*" := Red (at level 70).
 
-  (* one step reflexive parallel reduction relation *)
-  Inductive OneStepReflParRed : relation term :=
-    oneStepReflParRedK    u v       : OneStepReflParRed (K⋅u⋅v) u
-  | oneStepReflParRedS    u v w     : OneStepReflParRed (S⋅u⋅v⋅w) (u⋅w⋅(v⋅w))
-  | oneStepReflParRedRefl u         : OneStepReflParRed u u
-  | oneStepReflParRedPar  u u' v v' :
-      OneStepReflParRed u u' -> OneStepReflParRed v v' ->
-      OneStepReflParRed (u⋅v) (u'⋅v').
-  Local Infix ">>" := OneStepReflParRed (at level 70).
+  (**
+  ** One step reflexive parallel reduction relation
+  *)
 
-  (* reflexive parallel reduction relation *)
+  Local Reserved Infix ">>" (at level 70).
+  Inductive OneStepReflParRed : relation term :=
+  | oneStepReflParRedK    u v       : K⋅u⋅v >> u
+  | oneStepReflParRedS    u v w     : S⋅u⋅v⋅w >> u⋅w⋅(v⋅w)
+  | oneStepReflParRedRefl u         : u >> u
+  | oneStepReflParRedPar  u u' v v' : u >> u' -> v >> v' -> u⋅v >> u'⋅v'
+  where "u >> v" := (OneStepReflParRed u v).
+
+  (**
+  ** Reflexive parallel reduction relation
+  *)
+
   Definition ReflParRed := OneStepReflParRed+.
   Local Infix ">>*" := ReflParRed (at level 70).
 
-  (* relations between reduction relations *)
+  (**
+  ** Relations between reduction relations
+  *)
 
   Lemma inclusion1 : inclusion _ OneStepRed OneStepReflParRed.
   Proof. intros u v H. induction H; auto using OneStepReflParRed. Qed.
 
-  Lemma redL : forall u v u', u >* u' -> u⋅v >* u'⋅v.
+  Lemma redL (u v u' : term) : u >* u' -> u⋅v >* u'⋅v.
   Proof.
-    intros u v u' H.
-    induction H as [u u' | u | u w u' HL IHL HR IHR].
+    intro H. induction H as [u u' | u | u w u' HL IHL HR IHR].
     - apply rt_step. constructor. assumption.
     - apply rt_refl.
     - apply rt_trans with (y := w⋅v); assumption.
   Qed.
 
-  Lemma redR : forall u v v', v >* v' -> u⋅v >* u⋅v'.
+  Lemma redR (u v v' : term) : v >* v' -> u⋅v >* u⋅v'.
   Proof.
-    intros u v u' H. induction H as [v v' | v | v w v' HL IHL HR IHR].
+    intro H. induction H as [v v' | v | v w v' HL IHL HR IHR].
     - apply rt_step. constructor. assumption.
     - apply rt_refl.
     - apply rt_trans with (y := u⋅w); assumption.
   Qed.
 
-  Lemma redPar : forall u v u' v', u >* u' -> v >* v' -> u⋅v >* u'⋅v'.
+  Lemma redPar (u v u' v' : term) : u >* u' -> v >* v' -> u⋅v >* u'⋅v'.
   Proof.
-    intros u v u' v' Hu Hv.
+    intros Hu Hv.
     apply rt_trans with (y := u'⋅v); [apply redL | apply redR]; assumption.
   Qed.
 
@@ -98,39 +121,57 @@ Module TERM_PCA.
       + apply rt_trans with (y := w); assumption.
   Qed.
 
+  (**
+  ** The reduction relation is confluent
+  *)
+
   Lemma oneStepReflParRedDp : REL_RES.Dp _ OneStepReflParRed.
-  Proof with (eauto using OneStepReflParRed).
-    Ltac inj_subst H := injection H; intros; subst; clear H.
-    intros u v v' H. generalize dependent v'.
-    induction H as [v t | x y z | u | x x' y y' HL IHL HR IHR].
-    - remember (K⋅v⋅t) as u eqn:Hu.
-      intros v' H. destruct H.
-      + inj_subst Hu...
-      + inversion Hu.
-      + (* TODO (redundant case) *) admit.
-      + (* TODO (redundant case) *) admit.
-    - remember (S⋅x⋅y⋅z) as u eqn:Hu.
-      intros v' H'. destruct H'.
-      + (* TODO (redundant case) *) admit.
-      + inj_subst Hu...
-      + (* TODO (redundant case) *) admit.
-      + (* TODO (redundant case) *) admit.
-    - idtac...
-    - remember (x⋅y) as u eqn:Hu.
-      intros v' H. destruct H as [v' t | a b c | | x''' x'' y''' y'' HL' HR'].
-      + inj_subst Hu.
-        assert (exists v'', x' = K⋅v'' /\ v' >> v'') as [v'' [H H']].
-        { inversion_clear HL... inversion_clear H... }
-        subst...
-      + inj_subst Hu.
-        assert (exists a' b', x' = S⋅a'⋅b' /\ a >> a' /\ b >> b')
-          as [a' [b' [H [H' H'']]]].
-        { inversion_clear HL... inversion_clear H... inversion_clear H1... }
-        subst. exists (a'⋅y'⋅(b'⋅y'))...
-      + (* TODO (redundant case) *) admit.
-      + inj_subst Hu.
-        destruct (IHL x'' HL') as [x''' [H H']].
-        destruct (IHR y'' HR') as [y''' [H'' H''']]...
+  Proof.
+    (* redundant cases *)
+    assert (forall t u v, K⋅t >> u -> exists w, t >> w /\ u⋅v >> w) as case1. {
+      intros t u v H. inversion_clear H.
+      - eauto using OneStepReflParRed.
+      - inversion_clear H0. eauto using OneStepReflParRed.
+    }
+    assert
+      (forall u v w u' v',
+       S⋅u⋅v >> u' -> w >> v' -> exists w', u⋅w⋅(v⋅w) >> w' /\ u'⋅v' >> w')
+    as case2. {
+      intros u v w u' v' HL HR. remember (S⋅u⋅v) as Suv eqn:HSuv.
+      destruct HL as [u'' v'' | u'' v'' w'' | t | u'' u''' v'' v''' HL' HR'].
+      - inversion HSuv.
+      - discriminate HSuv.
+      - subst. eauto 6 using OneStepReflParRed.
+      - inj_subst HSuv. inversion_clear HL'.
+        + eauto 6 using OneStepReflParRed.
+        + inversion_clear H. eauto 6 using OneStepReflParRed.
+    }
+    (* the proof *)
+    intros t u v H. generalize dependent v.
+    induction H as [u v | u v w | t | u u' v v' HL IHL HR IHR].
+    - remember (K⋅u⋅v) as t eqn:Ht.
+      intros w H. destruct H as [u' v' | u' v' w' | t | u'' u' v'' v' H' H'' ].
+      + inj_subst Ht. eauto using OneStepReflParRed.
+      + inversion Ht.
+      + subst. eauto using OneStepReflParRed.
+      + inj_subst Ht. apply (case1 _ _ _ H').
+    - remember (S⋅u⋅v⋅w) as t eqn:Ht.
+      intros t' H.
+      destruct H as [u' v' | u' v' w' | t | u'' u' v'' v' H' H''].
+      + inversion Ht.
+      + inj_subst Ht. eauto using OneStepReflParRed.
+      + subst. eauto using OneStepReflParRed.
+      + inj_subst Ht. apply (case2 _ _ _ _  _ H' H'').
+    - eauto using OneStepReflParRed.
+    - remember (u⋅v) as t eqn:Ht.
+      intros t' H.
+      destruct H as [u'' v'' | u'' v'' w'' | t | u''' u'' v''' v'' HL' HR'].
+      + inj_subst Ht. pose proof (case1 _ _ v' HL). firstorder.
+      + inj_subst Ht. pose proof (case2 _ _ _ _ _ HL HR). firstorder.
+      + subst. eauto using OneStepReflParRed.
+      + inj_subst Ht.
+        destruct (IHL _ HL') as [u''' [H H']], (IHR _ HR') as [v''' [H'' H''']].
+        eauto using OneStepReflParRed.
   Qed.
 
   Theorem redConfluent : REL_RES.Dp _ Red.
@@ -146,105 +187,17 @@ Module TERM_PCA.
     + apply REL_RES.dp_confluence. apply oneStepReflParRedDp.
   Qed.
 
+  (**
+  ** Normal terms and normal forms
+  *)
+
   Definition Normal (u : term) := ~exists v, u > v.
 
-  Definition NormalForm (u v : term) := u >* v /\ Normal v.
-  Local Notation NF := NormalForm.
+  Lemma normApplL (u v : term) : Normal (u⋅v) -> Normal u.
+  Proof. intros H [t Ht]. eauto using OneStepRed. Qed.
 
-  Lemma normalRed : forall u v, Normal u -> u >* v -> u = v.
-  Proof.
-    intros n t H H'.
-    induction H' as [u v H' | u H' | u v w _ IHL _ IHR].
-    - exfalso. eauto.
-    - reflexivity.
-    - specialize (IHL H). subst. exact (IHR H).
-  Qed.
-
-  Theorem normalFormsUnique : forall u v v' : term, NF u v -> NF u v' -> v = v'.
-  Proof.
-    intros u v v' [Huv Hv] [Huv' Hv'].
-    destruct (redConfluent u v v' Huv Huv') as [w [Hvw Hv'w]].
-    apply normalRed in Hvw; [ | exact Hv].
-    apply normalRed in Hv'w; [ | exact Hv'].
-    congruence.
-  Qed.
-
-  Definition normalTerm := {t : term | Normal t}.
-
-  Definition normalTermsToTerms (t : normalTerm) : term :=
-    let (t, _) := t in t.
-
-  Local Coercion normalTermsToTerms : normalTerm >-> term.
-
-  Definition NormalTermEq (u v : normalTerm) := (u : term) = (v : term).
-
-  Instance normalTermEqEquivalence : Equivalence NormalTermEq.
-  Proof. unfold NormalTermEq. split; congruence. Qed.
-
-  Inductive StrictOneStepRed : term -> term -> Prop :=
-    strictOneStepRedConc u v w  :
-      Normal u -> Normal v -> u⋅v > w -> StrictOneStepRed (u⋅v) w
-  | strictOneStepRedL    u u' v :
-      StrictOneStepRed u u' -> StrictOneStepRed (u⋅v) (u'⋅v)
-  | strictOneStepRedR    u v v' :
-      StrictOneStepRed v v' -> StrictOneStepRed (u⋅v) (u⋅v').
-  Local Infix ">>>" := StrictOneStepRed (at level 70).
-
-  Definition StrictRed := StrictOneStepRed+.
-  Local Infix ">>>*" := StrictRed (at level 70).
-
-  Definition StrictNormalForm (u v : term) := u >>>* v /\ Normal v.
-  Local Notation SNF := StrictNormalForm.
-
-  Lemma strictOneStepRed_oneStepRed (u v : term) : u >>> v -> u > v.
-  Proof. intro H. induction H; auto using OneStepRed. Qed.
-
-  Lemma strictRed_red (u v : term) : u >>>* v -> u >* v.
-  Proof.
-    intro H. induction H as [u v | t | u v w _ IHL _ IHR].
-    - apply rt_step. apply strictOneStepRed_oneStepRed. exact H.
-    - apply rt_refl.
-    - apply rt_trans with (y := v); assumption.
-  Qed.
-
-  Lemma strictNormalForm_normalForm (u v : term) : SNF u v -> NF u v.
-  Proof. firstorder using strictRed_red. Qed.
-
-  Lemma strictNormalFormsUnique (u v w : term) : SNF u v -> SNF u w -> v = w.
-  Proof. eauto using strictNormalForm_normalForm, normalFormsUnique. Qed.
-
-  Definition NormalTermAppl (u v w : normalTerm) : Prop := SNF (u⋅v) w.
-
-  Lemma normalTermApplRespectful (u u' v v' w w' : normalTerm) :
-    NormalTermEq u u' -> NormalTermEq v v' -> NormalTermEq w w' ->
-    NormalTermAppl u v w -> NormalTermAppl u' v' w'.
-  Proof. unfold NormalTermEq, NormalTermAppl. congruence. Qed.
-
-  Instance normalTermApplProper :
-    Proper
-      (NormalTermEq ==> NormalTermEq ==> NormalTermEq ==> iff) NormalTermAppl.
-  Proof.
-    intros u u' Hu v v' Hv w w' Hw.
-    split;
-      [ | symmetry in Hu, Hv, Hw]; apply normalTermApplRespectful; assumption.
-  Qed.
-
-  Theorem normalTermApplFunctional (u v w w' : normalTerm) :
-    NormalTermAppl u v w -> NormalTermAppl u v w' -> NormalTermEq w w'.
-  Proof.
-    unfold NormalTermAppl, NormalTermEq. eauto using strictNormalFormsUnique.
-  Qed.
-
-  Instance termPas : PAS.Pas := {
-    carrier := normalTerm;
-    CarrierEq := NormalTermEq;
-    carrierEqEquivalence := normalTermEqEquivalence;
-    Appl := NormalTermAppl;
-    applRespectful := normalTermApplRespectful;
-    applFunctional := normalTermApplFunctional
-  }.
-
-  Local Open Scope PAS.
+  Lemma normApplR (u v : term) : Normal (u⋅v) -> Normal v.
+  Proof. intros H [t Ht]. eauto using OneStepRed. Qed.
 
   Lemma kNormal : Normal K.
   Proof. intros [u H]. inversion H. Qed.
@@ -273,7 +226,127 @@ Module TERM_PCA.
     - apply Hv. eauto.
   Qed.
 
-  Lemma normalConc (u v w w' : term) :
+  Definition NormalForm (u v : term) := u >* v /\ Normal v.
+  Local Notation NF := NormalForm.
+
+  Lemma normalRed (u v : term) : Normal u -> u >* v -> u = v.
+  Proof.
+    intros H H'.
+    induction H' as [u v H' | u H' | u v w _ IHL _ IHR].
+    - exfalso. eauto.
+    - reflexivity.
+    - specialize (IHL H). subst. exact (IHR H).
+  Qed.
+
+  Theorem normalFormsUnique (u v v' : term) : NF u v -> NF u v' -> v = v'.
+  Proof.
+    intros [Huv Hv] [Huv' Hv'].
+    destruct (redConfluent u v v' Huv Huv') as [w [Hvw Hv'w]].
+    apply normalRed in Hvw; [ | exact Hv].
+    apply normalRed in Hv'w; [ | exact Hv'].
+    congruence.
+  Qed.
+
+  (**
+  ** Strict one step reduction
+  *)
+
+  Local Reserved Infix ">>>" (at level 70).
+  Inductive StrictOneStepRed : term -> term -> Prop :=
+  | strictOneStepRedAppl u v w  : Normal u -> Normal v -> u⋅v > w -> u⋅v >>> w
+  | strictOneStepRedL    u u' v : u >>> u' -> u⋅v >>> u'⋅v
+  | strictOneStepRedR    u v v' : v >>> v' -> u⋅v >>> u⋅v'
+  where "u >>> v" := (StrictOneStepRed u v).
+
+  Lemma strictOneStepRed_oneStepRed (u v : term) : u >>> v -> u > v.
+  Proof. intro H. induction H; auto using OneStepRed. Qed.
+
+  (**
+  ** Strict reduction
+  *)
+
+  Definition StrictRed := StrictOneStepRed+.
+  Local Infix ">>>*" := StrictRed (at level 70).
+
+  Lemma strictRed_red (u v : term) : u >>>* v -> u >* v.
+  Proof.
+    intro H. induction H as [u v | t | u v w _ IHL _ IHR].
+    - apply rt_step. apply strictOneStepRed_oneStepRed. exact H.
+    - apply rt_refl.
+    - apply rt_trans with (y := v); assumption.
+  Qed.
+
+  Lemma strictRedL (u u' v : term) : u >>>* u' -> u⋅v >>>* u'⋅v.
+  Proof.
+    intro H. generalize dependent v.
+    induction H as [u u' H | u | u u' u'' _ IHL _ IHR]; intro v.
+    - apply rt_step. apply strictOneStepRedL. assumption.
+    - apply rt_refl.
+    - specialize (IHL v). specialize (IHR v).
+      apply rt_trans with (y := u'⋅v); assumption.
+  Qed.
+
+  Lemma strictRedR (u v v' : term) : v >>>* v' -> u⋅v >>>* u⋅v'.
+  Proof.
+    intro H. generalize dependent u.
+    induction H as [v v' H | v | v v' v'' _ IHL _ IHR]; intro u.
+    - apply rt_step. apply strictOneStepRedR. assumption.
+    - apply rt_refl.
+    - specialize (IHL u). specialize (IHR u).
+      apply rt_trans with (y := u⋅v'); assumption.
+  Qed.
+
+  Lemma strictRedPar (u u' v v' : term) :
+    u >>>* u' -> v >>>* v' -> u⋅v >>>* u'⋅v'.
+  Proof.
+    intros Hu Hv.
+    apply rt_trans with (y := u'⋅v);
+    [apply strictRedL | apply strictRedR]; assumption.
+  Qed.
+
+  (**
+  ** Strict normal forms
+  *)
+
+  Definition StrictNormalForm (u v : term) := u >>>* v /\ Normal v.
+  Local Notation SNF := StrictNormalForm.
+
+  Lemma strictNormalForm_normalForm (u v : term) : SNF u v -> NF u v.
+  Proof. firstorder using strictRed_red. Qed.
+
+  Lemma strictNormalFormsUnique (u v w : term) : SNF u v -> SNF u w -> v = w.
+  Proof. eauto using strictNormalForm_normalForm, normalFormsUnique. Qed.
+
+  (**
+  ** Normal terms form a partial applicative structure
+  *)
+
+  Definition normalTerm := {t : term | Normal t}.
+
+  Definition normalTermsToTerms (t : normalTerm) : term := proj1_sig t.
+  Local Coercion normalTermsToTerms : normalTerm >-> term.
+
+  Definition NormalTermEq (u v : normalTerm) := (u : term) = (v : term).
+
+  Instance normalTermEqEquivalence : Equivalence NormalTermEq.
+  Proof. unfold NormalTermEq. split; congruence. Qed.
+
+  Definition NormalTermAppl (u v w : normalTerm) : Prop := SNF (u⋅v) w.
+
+  Instance termPas : PAS.Pas := {
+    carrier := normalTerm;
+    CarrierEq := NormalTermEq;
+    carrierEqEquivalence := normalTermEqEquivalence;
+    Appl := NormalTermAppl
+  }.
+  Proof.
+    - unfold NormalTermAppl, NormalTermEq. congruence.
+    - unfold NormalTermAppl, NormalTermEq. eauto using strictNormalFormsUnique.
+  Defined.
+
+  Local Open Scope PAS.
+
+  Lemma normalApplRed (u v w w' : term) :
     Normal u -> Normal v -> u⋅v > w -> u⋅v > w' -> w = w'.
   Proof.
     intros Hu Hv H H'.
@@ -291,6 +364,10 @@ Module TERM_PCA.
     - exfalso. eauto.
     - exfalso. eauto.
   Qed.
+
+  (**
+  ** Strict one step reflexive reduction
+  *)
 
   Definition StrictOneStepReflRed :=
     REL_RES.ReflexiveClosure _ StrictOneStepRed.
@@ -312,91 +389,70 @@ Module TERM_PCA.
 
   Lemma strictOneStepReflRedDp : REL_RES.Dp _ StrictOneStepReflRed.
   Proof.
-    intros u v v' H H'. destruct H as [H | H]; destruct H' as [H' | H'].
-    - generalize dependent v'.
-      induction H as [u v w Hu Hv H | u_l u'_l u_r H IH | u_l u_r u'_r H IH].
-      + intros w' H'. remember (u⋅v) as uv eqn:Huv.
-        destruct H' as [u' v' w' Hu' Hv' H' | x v' y H' | ];
-        injection Huv; intros; subst; clear Huv.
-        * rewrite (normalConc u v w w' Hu Hv H H').
-          exists w'. split; right; reflexivity.
-        * exfalso. apply Hu. exists v'.
+    intros t u v H H'. destruct H as [H | H]; destruct H' as [H' | H'].
+    - generalize dependent v.
+      induction H as [u v w Hu Hv H | u u' v H IH | u v v' H IH].
+      + intros w' H'. remember (u⋅v) as t eqn:Ht.
+        destruct H' as [u' v' w' _ _ H' | u'' u' v' H' | u' v'' v' H'];
+        inj_subst Ht.
+        * rewrite (normalApplRed _ _ _ _ Hu Hv H H').
+          unfold StrictOneStepReflRed, REL_RES.ReflexiveClosure. eauto.
+        * exfalso. apply Hu. exists u'.
           apply strictOneStepRed_oneStepRed. assumption.
         * exfalso. apply Hv. exists v'.
           apply strictOneStepRed_oneStepRed. assumption.
-      + intros v' H'. remember (u_l⋅u_r) as a eqn:Ha.
-        destruct H' as [ | x u''_l y H' IH' | x y u'_r H'];
-        injection Ha; intros; subst; clear Ha.
-        * (* TODO: redundant case *) admit.
-        * destruct (IH u''_l H') as [w_l [H'' H''']]. exists (w_l⋅u_r).
-          split; apply strictOneStepReflRedL; assumption.
-        * exists (u'_l⋅u'_r).
+      + intros w H'. remember (u⋅v) as t eqn:Ht.
+        destruct H' as [u'' v'' w Hu _ H' | u''' u'' v''' H' | u'' v'' v' H'];
+        inj_subst Ht.
+        * exfalso. apply Hu. exists u'.
+          apply strictOneStepRed_oneStepRed. assumption.
+        * destruct (IH _ H') as [w [H'' H''']].
+          eauto using strictOneStepReflRedL.
+        * exists (u'⋅v').
           split; [apply strictOneStepReflRedR | apply strictOneStepReflRedL];
           left; assumption.
-      + intros v' H'. remember (u_l⋅u_r) as a eqn:Ha.
-        destruct H' as [ | | x y u''_r H'];
-        injection Ha; intros; subst; clear Ha.
-        * (* TODO: redundant case *) admit.
-        * (* TODO: redundant case *) admit.
-        * destruct (IH u''_r H') as [w_r [H'' H''']]. exists (u_l⋅w_r).
-          split; apply strictOneStepReflRedR; assumption.
-    - subst. exists v. split; [right | left]; auto.
-    - subst. exists v'. split; [left | right]; auto.
-    - exists u. subst. split; right; auto.
+      + intros w H'. remember (u⋅v) as t eqn:Ht.
+        destruct H' as [u'' v'' w _ Hv H' | u'' u' v''' H' | u' v''' v'' H'];
+        inj_subst Ht.
+        * exfalso. apply Hv. exists v'.
+          apply strictOneStepRed_oneStepRed. assumption.
+        * exists (u'⋅v').
+          split; [apply strictOneStepReflRedL | apply strictOneStepReflRedR];
+          left; assumption.
+        * destruct (IH _ H') as [w [H'' H''']].
+          eauto using strictOneStepReflRedR.
+    - subst. exists u. split; [right | left]; auto.
+    - subst. exists v. split; [left | right]; auto.
+    - exists t. subst. split; right; auto.
   Qed.
 
-  Lemma strictRedConfluence : REL_RES.Dp _ StrictRed.
+  (**
+  ** Strict reduction confluent
+  *)
+
+  Lemma strictRedConfluent : REL_RES.Dp _ StrictRed.
   Proof. apply REL_RES.dpReflClos_confluence. apply strictOneStepReflRedDp. Qed.
 
-  Lemma strictRedL : forall u u' v, u >>>* u' -> u⋅v >>>* u'⋅v.
-  Proof.
-    intros u u' v H. generalize dependent v.
-    induction H as [u u' H | u | u u' u'' _ IHL _ IHR]; intro v.
-    - apply rt_step. apply strictOneStepRedL. assumption.
-    - apply rt_refl.
-    - specialize (IHL v). specialize (IHR v).
-      apply rt_trans with (y := u'⋅v); assumption.
-  Qed.
-
-  Lemma strictRedR : forall u v v', v >>>* v' -> u⋅v >>>* u⋅v'.
-  Proof.
-    intros u v v' H. generalize dependent u.
-    induction H as [v v' H | v | v v' v'' _ IHL _ IHR]; intro u.
-    - apply rt_step. apply strictOneStepRedR. assumption.
-    - apply rt_refl.
-    - specialize (IHL u). specialize (IHR u).
-      apply rt_trans with (y := u⋅v'); assumption.
-  Qed.
-
-  Lemma strictRedPar : forall u u' v v', u >>>* u' -> v >>>* v' -> u⋅v >>>* u'⋅v'.
-  Proof.
-    intros u u' v v' Hu Hv.
-    apply rt_trans with (y := u'⋅v);
-    [apply strictRedL | apply strictRedR]; assumption.
-  Qed.
-
-  Lemma normConcL : forall n n', Normal (n⋅n') -> Normal n.
-  Proof.
-    intros n n' H [t Ht]. eauto using OneStepRed.
-  Qed.
-
-  Lemma normConcR : forall n n', Normal (n⋅n') -> Normal n'.
-  Proof.
-    intros n n' H [t Ht]. eauto using OneStepRed.
-  Qed.
+  (**
+  ** Strict one step left-or-right reduction
+  *)
 
   Reserved Notation "u >>>lr v" (at level 70, no associativity).
   Inductive StrictOneStepRedLeftRight : term -> term -> Prop :=
-    strictOneStepRedLeftRightL u u' v : u >>> u' -> u⋅v >>>lr u'⋅v
+  | strictOneStepRedLeftRightL u u' v : u >>> u' -> u⋅v >>>lr u'⋅v
   | strictOneStepRedLeftRightR u v v' : v >>> v' -> u⋅v >>>lr u⋅v'
   where "u >>>lr v" := (StrictOneStepRedLeftRight u v).
+
+  (**
+  ** Strict left-or-right reduction
+  *)
 
   Definition StrictRedLeftRight := StrictOneStepRedLeftRight+.
   Infix ">>>lr*" := StrictRedLeftRight (at level 70, no associativity).
 
-  Lemma strictRedLeftRightL : forall u v u' v', u⋅v >>>lr* u'⋅v' -> u >>>* u'.
+  Lemma strictRedLeftRightL (u v u' v' : term) : u⋅v >>>lr* u'⋅v' -> u >>>* u'.
   Proof.
-    intros u v u' v' H. apply REL_RES.nChain_clos_refl_trans in H.
+    intro H. apply REL_RES.nChain_clos_refl_trans in H.
     destruct H as [m H].
     generalize dependent v'. generalize dependent u'.
     generalize dependent v. generalize dependent u.
@@ -408,9 +464,9 @@ Module TERM_PCA.
       + eapply IH; eauto.
   Qed.
 
-  Lemma StrictRedLeftRightR : forall u v u' v', u⋅v >>>lr* u'⋅v' -> v >>>* v'.
+  Lemma strictRedLeftRightR (u v u' v' : term) : u⋅v >>>lr* u'⋅v' -> v >>>* v'.
   Proof.
-    intros u v u' v' H. apply REL_RES.nChain_clos_refl_trans in H.
+    intro H. apply REL_RES.nChain_clos_refl_trans in H.
     destruct H as [m H].
     generalize dependent v'. generalize dependent u'.
     generalize dependent v. generalize dependent u.
@@ -422,126 +478,134 @@ Module TERM_PCA.
         apply rt_step. assumption.
   Qed.
 
-  Lemma lemma : forall u v w, u⋅v >>>lr* w -> exists u' v', w = u'⋅v'.
-  Proof.
-    intros u v w H. apply REL_RES.nChain_clos_refl_trans in H.
-    destruct H as [m H].
-    generalize dependent w. generalize dependent v. generalize dependent u.
-    induction m as [ | m IH]; intros.
-    - inversion_clear H. eauto.
-    - inversion_clear H. specialize (IH u v b H0).
-      destruct IH as [u' [v' H]]. subst. destruct H1; eauto.
-  Qed.
+  (**
+  Closed PAS terms as terms
+  *)
 
-  Lemma lemma' : forall u v w, u⋅v >>>* w ->
-    u⋅v >>>lr* w
-    \/ exists n n', Normal n /\ Normal n' /\ u >>>* n /\ v >>>* n' /\ n⋅n' >>>* w.
-  Proof.
-    intros u v w H. apply REL_RES.nChain_clos_refl_trans in H.
-    destruct H as [m H].
-    generalize dependent w. generalize dependent v. generalize dependent u.
-    induction m as [ | m IH]; intros.
-    - inversion_clear H. left. apply rt_refl.
-    - inversion_clear H. specialize (IH u v b H0).
-      destruct IH as [IH | IH].
-      + inversion H1; subst.
-        * right. exists u0, v0. repeat split; auto.
-          { apply (strictRedLeftRightL _ _ _ _ IH). }
-          { apply (StrictRedLeftRightR _ _ _ _ IH). }
-          { apply rt_step. assumption. }
-        * left. eapply rt_trans; eauto. apply rt_step.
-          apply strictOneStepRedLeftRightL. assumption.
-        * left. eapply rt_trans; eauto. apply rt_step.
-          apply strictOneStepRedLeftRightR. assumption.
-      + right. destruct IH as [n [n' IH]]. exists n, n'.
-        repeat split; try tauto. apply rt_trans with (y := b); [tauto | ].
-        apply rt_step. assumption.
-  Qed.
-
-  Lemma lemma'' : forall u v n, u⋅v >>>* n -> Normal n -> exists n' n'',
-    SNF u n' /\ SNF v n'' /\ n'⋅n'' >>>* n.
-  Proof.
-    intros u v n H Hn. apply lemma' in H.
-    destruct H as [H | [n' [n'' [Hn' [Hn'' [H [H' H'']]]]]]].
-    - destruct (lemma u v n H) as [n' [n'' H']]. subst.
-      exists n', n''. split; [ | split].
-      + split; [ | apply (normConcL _ _ Hn)]. apply (strictRedLeftRightL _ _ _ _ H).
-      + split; [ | apply (normConcR _ _ Hn)]. apply (StrictRedLeftRightR _ _ _ _ H).
-      + apply rt_refl.
-    - exists n', n''. repeat split; auto.
-  Qed.
-
-  Fixpoint closedPasTermToTerm (t : @PAS.term termPas 0) : term := match t with
-  | &a            => let (a, _) := a in a
-  | PAS.termVar x => False_rect _ (FIN.t0Empty x)
-  | u*v           => closedPasTermToTerm u ⋅ closedPasTermToTerm v
+  Fixpoint closedPasTermToTerm (t : @PAS.term termPas 0) : term :=
+  match t with
+  | &a        => let (a, _) := a in a
+  | PAS.var x => False_rect _ (FIN.t0Empty x)
+  | u*v       => closedPasTermToTerm u ⋅ closedPasTermToTerm v
   end.
+  Local Notation "§ t" := (closedPasTermToTerm t) (at level 6).
 
-  Local Notation "$ t" := (closedPasTermToTerm t) (at level 6).
-
-  Lemma concatenationLemma (u : @PAS.term termPas 0) (v : normalTerm) :
-    $ u >>>* v -> u ≃ &v.
+  Lemma closedPasTermEq (u v : @PAS.term termPas 0) : §u >>>* §v -> u ≃ v.
   Proof.
-    generalize dependent v.
-    induction u as [u | x | u IHu v IHv].
-    - intros v H. simpl in H. apply strictRed_red in H.
-      cut (u == v); [intro H'; rewrite H'; reflexivity | ].
-      destruct u as [u Hu]. apply normalRed; assumption.
-    - destruct x.
-    - intros w H.
-      destruct (lemma'' _ _ _ H (proj2_sig w))
-        as [a [b [[H' Ha] [[H'' Hb] H''']]]].
-      fold closedPasTermToTerm in H', H''.
-      set (a' := exist _ _ Ha : normalTerm). setoid_rewrite (IHu a' H').
-      set (b' := exist _ _ Hb : normalTerm). setoid_rewrite (IHv b' H'').
-      setoid_rewrite PAS.correctness1'.
-      destruct w as [w Hw]. split; assumption.
-  Qed.
-
-  Lemma concatenationLemma' :
-    forall (u : @PAS.term termPas 0) (v : normalTerm), (u ≃ &v) <-> SNF $ u v.
-  Proof.
-    intro u. induction u as [u | x | u IHu v IHv].
-    - intro n. split; intro H.
-      + apply PAS.termConstInjective in H.
-        destruct u as [u Hu], n as [n Hn]. simpl in *.
-        unfold NormalTermEq in H. simpl in H. subst.
-        split; [apply rt_refl | exact Hn].
-      + cut (u == n); [intro Hun; rewrite Hun; reflexivity | ].
-        destruct H as [H _], u as [u Hu], n as [n Hn]. simpl in *.
-        unfold NormalTermEq. simpl.
-        apply normalRed; [exact Hu | ]. apply strictRed_red. exact H.
-    - inversion x.
-    - intro n. simpl. rewrite PAS.correctness1. split.
-      + intros [a [b [Hu [Hv H]]]].
-        specialize (IHu a).
-        specialize (IHv b).
-        destruct IHu as [IHu _]. specialize (IHu Hu). destruct IHu as [IHu _].
-        destruct IHv as [IHv _]. specialize (IHv Hv). destruct IHv as [IHv _].
-        unfold PAS.Appl in H. simpl in H. unfold NormalTermAppl in H.
-        destruct n as [n Hn]. destruct a as [a Ha]. destruct b as [b Hb].
-        simpl in *. split; [ | exact Hn].
-        destruct H as [H _].
-        apply rt_trans with (y := a⋅b); [ | exact H].
-        apply strictRedPar; assumption.
-      + intros [H Hn]. apply (concatenationLemma (u*v)) in H.
-        setoid_rewrite PAS.correctness1 in H. exact H.
-  Qed.
-
-  Lemma concatenationLemma'' (u v : @PAS.term termPas 0) :
-    $ u >>>* $ v -> u ≃ v.
-  Proof.
+    assert (forall u v w, u⋅v >>>lr* w -> exists u' v', w = u'⋅v') as lemma. {
+      clear.
+      intros u v w H. apply REL_RES.nChain_clos_refl_trans in H.
+      destruct H as [m H].
+      generalize dependent w. generalize dependent v. generalize dependent u.
+      induction m as [ | m IH]; intros.
+      - inversion_clear H. eauto.
+      - inversion_clear H. specialize (IH u v b H0).
+        destruct IH as [u' [v' H]]. subst. destruct H1; eauto.
+    }
+    assert
+      (forall u v w,
+       u⋅v >>>* w ->
+       u⋅v >>>lr* w \/
+       exists n n', Normal n /\ Normal n' /\ u >>>* n /\ v >>>* n'
+                    /\ n⋅n' >>>* w)
+    as lemma'. {
+      clear u v.
+      intros u v w H. apply REL_RES.nChain_clos_refl_trans in H.
+      destruct H as [m H].
+      generalize dependent w. generalize dependent v. generalize dependent u.
+      induction m as [ | m IH]; intros.
+      - inversion_clear H. left. apply rt_refl.
+      - inversion_clear H. specialize (IH u v b H0).
+        destruct IH as [IH | IH].
+        + inversion H1; subst.
+          * right. exists u0, v0. repeat split; auto.
+            { apply (strictRedLeftRightL _ _ _ _ IH). }
+            { apply (strictRedLeftRightR _ _ _ _ IH). }
+            { apply rt_step. assumption. }
+          * left. eapply rt_trans; eauto. apply rt_step.
+            apply strictOneStepRedLeftRightL. assumption.
+          * left. eapply rt_trans; eauto. apply rt_step.
+            apply strictOneStepRedLeftRightR. assumption.
+        + right. destruct IH as [n [n' IH]]. exists n, n'.
+          repeat split; try tauto. apply rt_trans with (y := b); [tauto | ].
+          apply rt_step. assumption.
+    }
+    assert
+      (forall u v n, u⋅v >>>* n -> Normal n ->
+                     exists n' n'', SNF u n' /\ SNF v n'' /\ n'⋅n'' >>>* n)
+    as lemma''. {
+      clear u v.
+      intros u v n H Hn. apply lemma' in H.
+      destruct H as [H | [n' [n'' [Hn' [Hn'' [H [H' H'']]]]]]].
+      - destruct (lemma u v n H) as [n' [n'' H']]. subst.
+        exists n', n''. split; [ | split].
+        + split; [ | apply (normApplL _ _ Hn)].
+          apply (strictRedLeftRightL _ _ _ _ H).
+        + split; [ | apply (normApplR _ _ Hn)].
+          apply (strictRedLeftRightR _ _ _ _ H).
+        + apply rt_refl.
+      - exists n', n''. repeat split; auto.
+    }
+    clear lemma lemma'.
+    assert (forall u (v : normalTerm), §u >>>* v -> u ≃ &v) as lemma. {
+      clear u v.
+      induction u as [u | x | u IHu v IHv].
+      - intros v H. simpl in H. apply strictRed_red in H.
+        cut (u == v); [intro H'; rewrite H'; reflexivity | ].
+        destruct u as [u Hu]. apply normalRed; assumption.
+      - destruct x.
+      - intros w H.
+        destruct (lemma'' _ _ _ H (proj2_sig w))
+          as [a [b [[H' Ha] [[H'' Hb] H''']]]].
+        fold closedPasTermToTerm in H', H''.
+        set (a' := exist _ _ Ha : normalTerm). setoid_rewrite (IHu a' H').
+        set (b' := exist _ _ Hb : normalTerm). setoid_rewrite (IHv b' H'').
+        setoid_rewrite PAS.correctness1'.
+        destruct w as [w Hw]. split; assumption.
+    }
+    assert (forall u (v : normalTerm), u ≃ &v <-> SNF §u v) as lemma'. {
+      clear u v.
+      intro u. induction u as [u | x | u IHu v IHv].
+      - intro n. split; intro H.
+        + apply PAS.constInjective in H.
+          destruct u as [u Hu], n as [n Hn]. simpl in *.
+          unfold NormalTermEq in H. simpl in H. subst.
+          split; [apply rt_refl | exact Hn].
+        + cut (u == n); [intro Hun; rewrite Hun; reflexivity | ].
+          destruct H as [H _], u as [u Hu], n as [n Hn]. simpl in *.
+          unfold NormalTermEq. simpl.
+          apply normalRed; [exact Hu | ]. apply strictRed_red. exact H.
+      - inversion x.
+      - intro n. simpl. rewrite PAS.correctness1. split.
+        + intros [a [b [Hu [Hv H]]]].
+          specialize (IHu a).
+          specialize (IHv b).
+          destruct IHu as [IHu _]. specialize (IHu Hu). destruct IHu as [IHu _].
+          destruct IHv as [IHv _]. specialize (IHv Hv). destruct IHv as [IHv _].
+          unfold PAS.Appl in H. simpl in H. unfold NormalTermAppl in H.
+          destruct n as [n Hn]. destruct a as [a Ha]. destruct b as [b Hb].
+          simpl in *. split; [ | exact Hn].
+          destruct H as [H _].
+          apply rt_trans with (y := a⋅b); [ | exact H].
+          apply strictRedPar; assumption.
+        + intros [H Hn]. apply (lemma (u*v)) in H.
+          setoid_rewrite PAS.correctness1 in H. exact H.
+    }
     intro H. apply PAS.correctness2. intro v'.
-    setoid_rewrite concatenationLemma'.
+    setoid_rewrite lemma'. clear lemma lemma' lemma''.
     split; intro H'; destruct H' as [H' _], v' as [v' Hv']; simpl in *.
     - split; [ | exact Hv'].
-      destruct (strictRedConfluence $ u $ v v' H H') as [w [H'' H''']].
+      destruct (strictRedConfluent §u §v v' H H') as [w [H'' H''']].
       assert (v' = w) as H4. {
         apply strictRed_red in H'''. apply normalRed in H'''; assumption.
       }
       subst. assumption.
-    - split; [ | exact Hv']. apply rt_trans with (y := $ v); assumption.
+    - split; [ | exact Hv']. apply rt_trans with (y := §v); assumption.
   Qed.
+
+  (**
+  ** Normal terms form a partial combinatory algebra
+  *)
 
   Definition k : normalTerm := exist _ _ kNormal.
   Definition s : normalTerm := exist _ _ sNormal.
@@ -552,22 +616,25 @@ Module TERM_PCA.
     s := s
   }.
   Proof.
-    - discriminate.
-    - intros [u Hu] [v Hv]. apply concatenationLemma''.
-      apply rt_step. simpl. apply strictOneStepRedConc.
+    - intros [u Hu] [v Hv]. apply closedPasTermEq.
+      apply rt_step. simpl. apply strictOneStepRedAppl.
       + apply ktNormal. exact Hu.
       + exact Hv.
       + apply oneStepRedK.
     - intros [u Hu] [v Hv].
       set (suv := exist _ _ (suvNormal _ _ Hu Hv) : normalTerm).
-      exists suv. apply concatenationLemma''. apply rt_refl.
+      exists suv. apply closedPasTermEq. apply rt_refl.
     - intros [u Hu] [v Hv] [w Hw].
-      apply concatenationLemma''. simpl.
-      apply rt_step. apply strictOneStepRedConc.
+      apply closedPasTermEq. simpl.
+      apply rt_step. apply strictOneStepRedAppl.
       + apply suvNormal; assumption.
       + exact Hw.
       + apply oneStepRedS.
-  Qed.
+  Defined.
+
+  (**
+  ** Notations
+  *)
 
   Module NOTATIONS.
 
@@ -577,18 +644,17 @@ Module TERM_PCA.
       (fun u v => u ⋅ v) (at level 40, left associativity) : TERM_PCA.
     Infix ">" := (fun u v => u > v) (at level 70) : TERM_PCA.
     Infix ">*" := (fun u v => u >* v) (at level 70) : TERM_PCA.
-    Infix ">>" := (fun u v => u >> v) (at level 70) : TERM_PCA.
-    Infix ">>*" := (fun u v => u >>* v) (at level 70) : TERM_PCA.
-    Infix ">>=" := (fun u v => u >>= v) (at level 70) : TERM_PCA.
     Infix ">>>" := (fun u v => u >>> v) (at level 70) : TERM_PCA.
     Infix ">>>*" := (fun u v => u >>>* v) (at level 70) : TERM_PCA.
-    Infix ">>>lr" := (fun u v => u >>>lr v) (at level 70) : TERM_PCA.
-    Infix ">>lr*" := (fun u v => u >>>lr* v) (at level 70) : TERM_PCA.
-    Notation "$ t" := ($ t) (at level 6) : TERM_PCA.
+    Notation "§ t" := (§t) (at level 6) : TERM_PCA.
 
   End NOTATIONS.
 
 End TERM_PCA.
+
+(**
+** Coercions
+*)
 
 Module TERM_PCA_COERCIONS.
   Import TERM_PCA.
