coq/fin.v
@@ -1,0 +1,87 @@
+(**
+* Canonical finite types
+[FIN.t n] is a type with [n] members,
+one member naturally corresponding to each [m < n].
+*)
+
+Module FIN.
+
+  (**
+  ** Definition
+  [t 0] is the empty type.
+  [t (S n)] is the sum of
+  [t n] and the singleton of [n].
+  *)
+
+  Inductive Singleton (n : nat) := lift : Singleton n.
+
+  Fixpoint t (n : nat) : Type :=
+  match n with
+  | O   => Empty_set
+  | S n => sum (t n) (Singleton n)
+  end.
+
+  Definition last {n} : t (S n) := inr (lift n).
+
+  Lemma t0Empty (x : t 0) : False.
+  Proof. destruct x. Qed.
+
+  Lemma t1Singleton (x : t 1) : x = last.
+  Proof. destruct x as [x | x]; destruct x. reflexivity. Qed.
+
+  (**
+  An element of
+  [FIN.t n]
+  is also an element of
+  [FIN.t (S n)].
+  More generally,
+  it is also an element of
+  [FIN.t (k + n)].
+  *)
+
+  Definition up {n} (x : t n) : t (S n) := inl x.
+  Local Notation "++ x" := (up x) (at level 6, right associativity).
+
+  Fixpoint up' {n k} (x : t n) : t (k + n) :=
+  match k with
+  | O   => x
+  | S k => ++(up' x)
+  end.
+
+  (**
+  ** Functions to and from naturals
+  *)
+
+  Definition ofNat (n k : nat) : t (k + S n) := up' last.
+
+  Fixpoint toNat {n} : t (S n) -> nat :=
+  match n with
+  | O   => fun x => 0
+  | S n => fun x => match x with
+                    | inl x => toNat x
+                    | inr x => n
+                    end
+  end.
+
+  (**
+  Now one would want to prove
+  the correctness of [ofNat] and [toNat],
+  i.e. that [ofNat (toNat x) k = up' x] and
+  that [toNat (ofNat n k) = n].
+  It is however nontrivial to even state these,
+  since [(k + S n) = (S _)] does not automatically typecheck.
+  For my purposes,
+  I do not need to prove their correctness so
+  I will skip doing so.
+  *)
+
+  (**
+  ** Notations
+  *)
+
+  Module NOTATIONS.
+    Delimit Scope FIN with FIN.
+    Notation "++ x" := ++x (at level 6, right associativity) : FIN.
+  End NOTATIONS.
+
+End FIN.
