coq/relationresults.v
@@ -1,3 +1,10 @@
+(**
+* Some results on relation operators
+Taken from
+``Polishing up the Tait--Martin-Lof proof of the Church-Rosser theorem''
+(Robert Pollack 1995).
+*)
+
 Require Import Relations.
 Require Import Relation_Operators.
 
@@ -10,34 +17,89 @@ Module REL_RES.
     Variable A : Type.
     Local Notation Rel := (relation A).
 
-    (* generalized diamond property *)
+    (**
+    ** Definitions
+    *)
+
+    (**
+    *** Reflexive closure
+    *)
+
+    Definition ReflexiveClosure (R : Rel) a b := R a b \/ a = b.
+
+    (**
+    *** Generalized diamond property
+    *)
+
     Definition Gdp (R S : Rel) : Prop :=
       forall a b b', R a b -> S a b' -> exists c : A, S b c /\ R b' c.
 
-    (* diamond property *)
+    (**
+    *** Diamond property
+    *)
+
     Definition Dp (R : Rel) : Prop := Gdp R R.
 
-    (* commutativity of generalized diamond property *)
-    Lemma generalizedDiamondCommutative (R S : Rel) : Gdp R S -> Gdp S R.
-    Proof. intros H a b c H' H''. specialize (H a c b H'' H'). firstorder. Qed.
+    (**
+    *** Confluence
+    *)
 
-    (* strip property *)
+    Definition Confluence (R : relation A) := Dp R+.
+
+    (**
+    *** Strip property
+    *)
+
     Definition strip (f : Rel -> Rel) :=
       forall R S : Rel, Gdp R S -> Gdp R (f S).
 
-    (* strips property *)
+    (**
+    *** Strips property
+    *)
+
     Definition strips (f : relation A -> relation A) :=
       forall R S : Rel, Gdp R S -> Gdp (f R) (f S).
 
-    (* strip implies strips *)
-    Lemma strip_strips (f : Rel -> Rel) : strip f -> strips f.
-    Proof. unfold strips. auto using generalizedDiamondCommutative. Qed.
+    (**
+    *** Relation chains
+    The [R]-chain of length [n] relates two elements [a0] and [an]
+    if there is [a_1,...,a(n-1)] such that
+    [a0Ra1R...Ra(n-1)Ran].
+    *)
 
-    (* transitive reflexive closure is extensive *)
+    Inductive nChain (R : Rel) : nat -> A -> A -> Prop :=
+    | nChain0 a       : nChain R 0 a a
+    | nChainS n a b c : nChain R n a b -> R b c -> nChain R (S n) a c.
+
+    (**
+    ** Results
+    *)
+
+    (**
+    *** Commutativity of generalized diamond property
+    *)
+
+    Lemma gdpCommutative (R S : Rel) : Gdp R S -> Gdp S R.
+    Proof. intros H a b c H' H''. specialize (H a c b H'' H'). firstorder. Qed.
+
+    (**
+    *** Strip property implies strips property
+    *)
+
+    Lemma strip_strips (f : Rel -> Rel) : strip f -> strips f.
+    Proof. unfold strips. auto using gdpCommutative. Qed.
+
+    (**
+    *** Transitive reflexive closure is extensive
+    *)
+
     Lemma clos_refl_transExtensive (R : Rel) : inclusion _ R R+.
     Proof. unfold inclusion. auto using rt_step. Qed.
 
-    (* transitive reflexive closure is increasing *)
+    (**
+    *** Transitive reflexive closure is increasing
+    *)
+
     Lemma clos_refl_transIncreasing (R S : Rel) :
       inclusion _ R S -> inclusion _ R+ S+.
     Proof.
@@ -46,12 +108,15 @@ Module REL_RES.
         [auto using rt_step | apply clos_rt_is_preorder | eauto using rt_trans].
     Qed.
 
-    (* the transitive reflexive closure has the strip property *)
+    (**
+    *** Transitive reflexive closure has the strip property
+    *)
+
     Lemma clos_refl_transStrip : strip (clos_refl_trans A).
     Proof.
       intros R S H.
-      apply generalizedDiamondCommutative.
-      apply generalizedDiamondCommutative in H.
+      apply gdpCommutative.
+      apply gdpCommutative in H.
       intros a b c H'. generalize dependent c.
       induction H' as [a b H' | a | a b' b HL IHL HR IHR].
       - intros c H''.
@@ -62,12 +127,16 @@ Module REL_RES.
         destruct (IHR b'' H'') as [d [H4 H5]]. eauto using rt_trans.
     Qed.
 
-    Definition Confluence (R : relation A) := Dp R+.
+    (**
+    *** Diamond property implies confluence
+    *)
 
     Theorem dp_confluence (R : Rel) : Dp R -> Confluence R.
     Proof. apply strip_strips. apply clos_refl_transStrip. Qed.
 
-    Definition ReflexiveClosure (R : Rel) a b := R a b \/ a = b.
+    (**
+    *** Diamond property of reflexive closure implies confluence
+    *)
 
     Theorem dpReflClos_confluence (R : Rel) :
       Dp (ReflexiveClosure R) -> Confluence R.
@@ -91,14 +160,13 @@ Module REL_RES.
       apply H in Hvw. apply H in Hv'w. eauto.
     Qed.
 
-    Inductive nChain (R : Rel) : nat -> A -> A -> Prop :=
-    | nChain0 a       : nChain R 0 a a
-    | nChainS n a b c : nChain R n a b -> R b c -> nChain R (S n) a c.
+    (**
+    *** Equivalence between reflexive transitive closure and chains
+    *)
 
-    Theorem nChain_clos_refl_trans :
-      forall R a b, R+ a b <-> exists n, nChain R n a b.
+    Theorem nChain_clos_refl_trans R a b : R+ a b <-> exists n, nChain R n a b.
     Proof.
-      intros R a b. split; intro H.
+      split; intro H.
       - induction H as [a b H | a | a b c HL [n IHL] HR [m IHR]].
         + exists 1. apply nChainS with (b := a); [constructor | assumption].
         + exists 0. constructor.
@@ -118,12 +186,13 @@ Module REL_RES.
 
   End RelationResults.
 
+  (**
+  ** Notations
+  *)
+
   Module NOTATIONS.
-
     Delimit Scope REL_RES with REL_RES.
-
     Notation "R +" := R+ (at level 5) : REL_RES.
-
   End NOTATIONS.
 
 End REL_RES.
