coq/vec.v
@@ -1,0 +1,234 @@
+(**
+* A vector library
+I am probably more or less reinventing the wheel here,
+but I found the standard library's vector implementations
+([Coq.Vectors.*])
+insufficient for two reasons.
+The first reason is that
+vectors are defined as separate inductive types,
+instead of as functions to [Type],
+with which a lot would come for free by computation
+and with which induction proofs would be easier.
+The second reason is that
+all functions are defined under the interpretation that
+vectors are built by appending a vector to an element.
+For my purposes the reverse interpretation---that
+vectors are built by appending an element to a vector---is
+more suitable.
+*)
+
+Require Import Coq.Classes.Morphisms.
+
+Require Import fin.
+
+Import FIN.NOTATIONS.
+Local Open Scope FIN.
+
+Module VEC.
+
+  (**
+  ** Definition
+  For each type [A],
+  there is one [A]-vector of length [0]---the empty vector---and
+  the type of [A]-vectors of length [S n] is
+  the product of the type of [A]-vectors of length [n] and [A].
+  *)
+
+  Inductive Empty (A : Type) := empty.
+  Arguments empty {_}.
+
+  Fixpoint t A (n : nat) : Type :=
+  match n with
+  | O   => Empty A
+  | S n => prod (t A n) A
+  end.
+  Local Notation "()" := (empty : t _ 0).
+  Local Infix ";;" :=
+    ((fun A n (v : t A n) (a : A) => ((v, a) : t A (S n))) _ _)
+    (at level 40, left associativity).
+
+  (**
+  ** Accessing elements of a vector
+  *)
+
+  Fixpoint nth {A} {n} : t A n -> FIN.t n -> A :=
+  match n with
+  | O   => fun _ x => False_rect _ (FIN.t0Empty x)
+  | S n => fun v x => let (v, a) := v in
+                      match x with
+                      | inl x => nth v x
+                      | inr _ => a
+                      end
+  end.
+
+  (**
+  ** Equality is pointwise equality
+  *)
+
+  Lemma pointwiseEquality {A} {n} (v w : t A n) :
+    v = w <-> (forall x : FIN.t n, nth v x = nth w x).
+  Proof.
+    split; [intro; subst; tauto | ].
+    intro H.
+    induction n as [ | n IHn].
+    - destruct v, w. reflexivity.
+    - destruct v as [v a], w as [w b].
+      specialize (IHn v w).
+      pose proof (H FIN.last) as H'. simpl in H'. rewrite H'. clear H'.
+      lapply IHn; [intro; subst; tauto | ]. clear IHn.
+      intro x. exact (H ++x).
+  Qed.
+
+  (**
+  ** Vectors of copies of an element
+  *)
+
+  Fixpoint copies {A} (n : nat) (a : A) : t A n :=
+  match n with
+  | O   => ()
+  | S n => (copies n a, a)
+  end.
+
+  Lemma nthCopiesEq {A} {n} (a : A) (x : FIN.t n) : nth (copies n a) x = a.
+  Proof.
+    induction n as [ | n IHn]; simpl.
+    - inversion x.
+    - destruct x as [x | x].
+      + apply IHn.
+      + reflexivity.
+  Qed.
+
+  (**
+  ** Concatenation of vectors
+  *)
+
+  Fixpoint concat {A} {n m} (v : t A n) : t A m -> t A (m + n) :=
+  match m with
+  | O   => fun _ => v
+  | S m => fun w => let (w, a) := w in (concat v w, a)
+  end.
+
+  (**
+  ** Mapping functions on vectors
+  The map of
+  [f : A -> B]
+  over an [A]-vector
+  [((), a1, a2, .., an)]
+  is the [B]-vector
+  [((), f a1, f a2, ..., f an)].
+  *)
+
+  Fixpoint map {A B} {n} (f : A -> B) : t A n -> t B n :=
+  match n with
+  | O   => fun _ => ()
+  | S n => fun v => let (v, a) := v in (map f v, f a)
+  end.
+
+  Lemma mapRespectful {A B} {n} (f g : A -> B) (v : t A n) :
+    (forall a : A, f a = g a) -> map f v = map g v.
+  Proof.
+    intro H.
+    induction n as [ | n IHn].
+    - reflexivity.
+    - destruct v as [v a]. simpl. rewrite IHn, H. reflexivity.
+  Qed.
+
+  Instance mapProper {A B} {n} :
+    Proper ((fun f g => forall a : A, f a = g a) ==> eq ==> eq) (@map A B n).
+  Proof. intros f g Hfg v w Hvw. subst. apply mapRespectful. exact Hfg. Qed.
+
+  Lemma mapComposeEq {A B C} {n} (f : A -> B) (g : B -> C) (v : t A n) :
+    map g (map f v) = map (fun a => g (f a)) v.
+  Proof.
+    induction n as [ | n IHn].
+    - reflexivity.
+    - destruct v as [v a]. simpl. rewrite IHn. reflexivity.
+  Qed.
+
+  Lemma nthMapEq {A B} {n} (f : A -> B) (v : t A n) (x : FIN.t n) :
+    nth (map f v) x = f (nth v x).
+  Proof.
+    induction n as [ | n IHn].
+    - inversion x.
+    - destruct v as [v a]. destruct x as [x | x].
+      + apply IHn.
+      + reflexivity.
+  Qed.
+
+  Lemma mapConcatEq {A B} {n m} (f : A -> B) (v : VEC.t A n) (w : VEC.t A m) :
+    map f (concat v w) = concat (map f v) (map f w).
+  Proof.
+    induction m as [ | m IHm]; simpl.
+    - reflexivity.
+    - destruct w as [w a]. rewrite IHm. reflexivity.
+  Qed.
+
+  (**
+  ** Vectors as the image of functions on the canonically finite sets
+  *)
+
+  Fixpoint finMap {A} {n} : (FIN.t n -> A) -> t A n :=
+  match n with
+  | O   => fun _ => ()
+  | S n => fun f => (finMap (fun x => f ++x), f FIN.last)
+  end.
+
+  Lemma nthFinMapEq {A} {n} (f : FIN.t n -> A) (x : FIN.t n) :
+    VEC.nth (finMap f) x = f x.
+  Proof.
+    induction n as [ | n IHn].
+    - inversion x.
+    - destruct x as [x | x]; simpl.
+      + rewrite IHn. reflexivity.
+      + destruct x. reflexivity.
+  Qed.
+
+  Lemma finMapComposeEq {A B} {n} (f : FIN.t n -> A) (g : A -> B) :
+    map g (finMap f) = finMap (fun x => g (f x)).
+  Proof.
+    induction n as [ | n IHn].
+    - reflexivity.
+    - simpl. rewrite IHn. reflexivity.
+  Qed.
+
+  Definition finMap' {A} {n k} (f : FIN.t (k + n) -> A) : t A n :=
+    finMap (fun x => f (FIN.up' x)).
+
+  Lemma nthFinMapEq' {A} {n k} (f : FIN.t (k + n) -> A) (x : FIN.t n) :
+    VEC.nth (finMap' f) x = f (FIN.up' x).
+  Proof. unfold finMap'. rewrite nthFinMapEq. reflexivity. Qed.
+
+  Lemma finMapComposeEq' {A B} {n k} (f : FIN.t (k+n) -> A) (g : A -> B) :
+    map g (finMap' f) = finMap' (fun x => g (f x)).
+  Proof. unfold finMap'. apply finMapComposeEq. Qed.
+
+  (**
+  ** Left fold
+  *)
+
+  Fixpoint foldl {A} {n} (f : A -> A -> A) : A -> t A n -> A :=
+  match n with
+  | O   => fun a _ => a
+  | S n => fun a v => let (v, b) := v in f (foldl f a v) b
+  end.
+
+  Lemma foldlConcatEq {A} {n m} (f : A -> A -> A) (a : A) (v : t A n)
+                      (w : t A m) :
+    foldl f a (concat v w) = foldl f (foldl f a v) w.
+  Proof.
+    induction m as [ | m IHm]; simpl.
+    - reflexivity.
+    - destruct w as [w b]. rewrite IHm. reflexivity.
+  Qed.
+
+  (**
+  ** Notations
+  *)
+
+  Module NOTATIONS.
+    Delimit Scope VEC with VEC.
+    Notation "()" := () : VEC.
+    Infix ";;" := (fun v a => v;; a) (at level 40, left associativity) : VEC.
+  End NOTATIONS.
+
+End VEC.
